{
  "schema_version": "1.0",
  "epd": {
    "id": "EPD-IES-20602:001",
    "source_pdf": "epd-ies-20602-001-holcim-vic-melbourne-metro-ecopact-ve322eamf-epd.pdf",
    "pages": 20,
    "program_operator": "EPD International AB (The International EPD System); Regional Programme: EPD Australasia",
    "pcr": "PCR 2019:14 Construction Products, Version 1.3.4, 2024-04-30; c-PCR-003 Concrete and Concrete Elements, 2024-04-30",
    "reference_standard": "EN 15804:2012+A2:2019/AC:2021 (ISO 14025)",
    "en15804_version": "A2",
    "characterisation": "EF 3.1",
    "published": "2025-04-15",
    "valid_until": "2030-04-15",
    "provenance": {
      "program_operator": {
        "page": 1,
        "snippet": "Programme operator: EPD International AB"
      },
      "pcr": {
        "page": 2,
        "snippet": "Product category rules | PCR 2019:14 Construction Products, Version 1.3.4, 2024-04-30"
      },
      "published": null,
      "valid_until": {
        "page": 2,
        "snippet": "Valid Until\n15/04/2030"
      }
    },
    "page_labels": null
  },
  "products": [
    {
      "name": "VIC - Melbourne Metro - ECOPact - VE322EAMF (S32@56D 20mm 120SL ECOPactMAX FIB CONC)",
      "manufacturer": "Holcim (Australia) Pty Ltd",
      "concrete_type": "Ready-mix concrete",
      "compressive_strength": {
        "value_mpa": 32,
        "class": "S32",
        "at_days": 56,
        "raw": "Strength (MPa) 32.0 | Mix Code VE322EAMF | Mix Description S32@56D 20mm 120SL ECOPactMAX FIB CONC",
        "status": "found",
        "provenance": {
          "page": 10,
          "snippet": "Strength (MPa) 32.0 VE322EAMF S32@56D 20mm 120SL ECOPactMAX FIB CONC General"
        }
      },
      "manufacturing_location": {
        "site": "Melbourne Metro network of Holcim batching plants",
        "city": "Melbourne (Laverton, Truganina, Footscray, Epping, Keilor, Preston, etc.)",
        "region": "VIC",
        "country": "AU",
        "raw": "Production Sites: Laverton, Truganina, Footscray, Epping, Keilor, Preston, Oaklands Junction, Melbourne Airport, Bayswater, Springvale, Lyndhurst, Seaford, Pakenham, Hastings, Rosebud",
        "provenance": {
          "page": 10,
          "snippet": "Production Sites Laverton, Truganina, Footscray, Epping, Keilor, Preston, Oaklands Junction, Melbourne Airport, Bayswater, Springvale, Lyndhurst, Seaford, Pakenham, Hastings, Rosebud"
        },
        "note": "Multi-plant Melbourne Metro EPD. The page-6 'Address and Contact Information' (100 Miller St, North Sydney) is the corporate/EPD-owner HQ, not a production site."
      },
      "declared_unit": {
        "amount": 1,
        "unit": "m3",
        "description": "1 m3 of ready-mix concrete.",
        "mass_kg": 2400,
        "provenance": {
          "page": 6,
          "snippet": "Declared Unit 1 m3 of ready-mix concrete."
        }
      },
      "indicators": {
        "GWP_total": {
          "unit_raw": "kg CO2 eq",
          "unit_normalised": "kg CO2e",
          "header_modules": [
            "A1-A3",
            "A4",
            "A5",
            "C1",
            "C2",
            "C3",
            "C4",
            "D"
          ],
          "modules": {
            "A1-A3": {
              "value": 105.0,
              "raw": "105",
              "status": "declared",
              "provenance": {
                "page": 15,
                "section": "",
                "table": "",
                "module": "A1-A3",
                "unit_raw": "kg CO2 eq"
              }
            },
            "A4": {
              "value": 2.05,
              "raw": "2.05",
              "status": "declared",
              "provenance": {
                "page": 15,
                "section": "",
                "table": "",
                "module": "A4",
                "unit_raw": "kg CO2 eq"
              }
            },
            "A5": {
              "value": 8.81,
              "raw": "8.81",
              "status": "declared",
              "provenance": {
                "page": 15,
                "section": "",
                "table": "",
                "module": "A5",
                "unit_raw": "kg CO2 eq"
              }
            },
            "C1": {
              "value": 0.532,
              "raw": "0.532",
              "status": "declared",
              "provenance": {
                "page": 15,
                "section": "",
                "table": "",
                "module": "C1",
                "unit_raw": "kg CO2 eq"
              }
            },
            "C2": {
              "value": 3.99,
              "raw": "3.99",
              "status": "declared",
              "provenance": {
                "page": 15,
                "section": "",
                "table": "",
                "module": "C2",
                "unit_raw": "kg CO2 eq"
              }
            },
            "C3": {
              "value": 7.61,
              "raw": "7.61",
              "status": "declared",
              "provenance": {
                "page": 15,
                "section": "",
                "table": "",
                "module": "C3",
                "unit_raw": "kg CO2 eq"
              }
            },
            "C4": {
              "value": 1.28,
              "raw": "1.28",
              "status": "declared",
              "provenance": {
                "page": 15,
                "section": "",
                "table": "",
                "module": "C4",
                "unit_raw": "kg CO2 eq"
              }
            },
            "D": {
              "value": -15.7,
              "raw": "-15.7",
              "status": "declared",
              "provenance": {
                "page": 15,
                "section": "",
                "table": "",
                "module": "D",
                "unit_raw": "kg CO2 eq"
              }
            }
          }
        },
        "GWP_fossil": {
          "unit_raw": "kg CO2 eq",
          "unit_normalised": "kg CO2e",
          "header_modules": [
            "A1-A3",
            "A4",
            "A5",
            "C1",
            "C2",
            "C3",
            "C4",
            "D"
          ],
          "modules": {
            "A1-A3": {
              "value": 104.0,
              "raw": "104",
              "status": "declared",
              "provenance": {
                "page": 15,
                "section": "",
                "table": "",
                "module": "A1-A3",
                "unit_raw": "kg CO2 eq"
              }
            },
            "A4": {
              "value": 2.05,
              "raw": "2.05",
              "status": "declared",
              "provenance": {
                "page": 15,
                "section": "",
                "table": "",
                "module": "A4",
                "unit_raw": "kg CO2 eq"
              }
            },
            "A5": {
              "value": 8.79,
              "raw": "8.79",
              "status": "declared",
              "provenance": {
                "page": 15,
                "section": "",
                "table": "",
                "module": "A5",
                "unit_raw": "kg CO2 eq"
              }
            },
            "C1": {
              "value": 0.532,
              "raw": "0.532",
              "status": "declared",
              "provenance": {
                "page": 15,
                "section": "",
                "table": "",
                "module": "C1",
                "unit_raw": "kg CO2 eq"
              }
            },
            "C2": {
              "value": 3.99,
              "raw": "3.99",
              "status": "declared",
              "provenance": {
                "page": 15,
                "section": "",
                "table": "",
                "module": "C2",
                "unit_raw": "kg CO2 eq"
              }
            },
            "C3": {
              "value": 7.6,
              "raw": "7.60",
              "status": "declared",
              "provenance": {
                "page": 15,
                "section": "",
                "table": "",
                "module": "C3",
                "unit_raw": "kg CO2 eq"
              }
            },
            "C4": {
              "value": 1.28,
              "raw": "1.28",
              "status": "declared",
              "provenance": {
                "page": 15,
                "section": "",
                "table": "",
                "module": "C4",
                "unit_raw": "kg CO2 eq"
              }
            },
            "D": {
              "value": -15.7,
              "raw": "-15.7",
              "status": "declared",
              "provenance": {
                "page": 15,
                "section": "",
                "table": "",
                "module": "D",
                "unit_raw": "kg CO2 eq"
              }
            }
          }
        },
        "GWP_biogenic": {
          "unit_raw": "kg CO2 eq",
          "unit_normalised": "kg CO2e",
          "header_modules": [
            "A1-A3",
            "A4",
            "A5",
            "C1",
            "C2",
            "C3",
            "C4",
            "D"
          ],
          "modules": {
            "A1-A3": {
              "value": 0.781,
              "raw": "0.781",
              "status": "declared",
              "provenance": {
                "page": 15,
                "section": "",
                "table": "",
                "module": "A1-A3",
                "unit_raw": "kg CO2 eq"
              }
            },
            "A4": {
              "value": 0.000153,
              "raw": "0.000153",
              "status": "declared",
              "provenance": {
                "page": 15,
                "section": "",
                "table": "",
                "module": "A4",
                "unit_raw": "kg CO2 eq"
              }
            },
            "A5": {
              "value": 0.024,
              "raw": "0.0240",
              "status": "declared",
              "provenance": {
                "page": 15,
                "section": "",
                "table": "",
                "module": "A5",
                "unit_raw": "kg CO2 eq"
              }
            },
            "C1": {
              "value": 4.09e-05,
              "raw": "0.0000409",
              "status": "declared",
              "provenance": {
                "page": 15,
                "section": "",
                "table": "",
                "module": "C1",
                "unit_raw": "kg CO2 eq"
              }
            },
            "C2": {
              "value": 0.000299,
              "raw": "0.000299",
              "status": "declared",
              "provenance": {
                "page": 15,
                "section": "",
                "table": "",
                "module": "C2",
                "unit_raw": "kg CO2 eq"
              }
            },
            "C3": {
              "value": 0.00704,
              "raw": "0.00704",
              "status": "declared",
              "provenance": {
                "page": 15,
                "section": "",
                "table": "",
                "module": "C3",
                "unit_raw": "kg CO2 eq"
              }
            },
            "C4": {
              "value": 0.00023,
              "raw": "0.000230",
              "status": "declared",
              "provenance": {
                "page": 15,
                "section": "",
                "table": "",
                "module": "C4",
                "unit_raw": "kg CO2 eq"
              }
            },
            "D": {
              "value": -0.0216,
              "raw": "-0.0216",
              "status": "declared",
              "provenance": {
                "page": 15,
                "section": "",
                "table": "",
                "module": "D",
                "unit_raw": "kg CO2 eq"
              }
            }
          }
        },
        "GWP_luluc": {
          "unit_raw": "kg CO2 eq",
          "unit_normalised": "kg CO2e",
          "header_modules": [
            "A1-A3",
            "A4",
            "A5",
            "C1",
            "C2",
            "C3",
            "C4",
            "D"
          ],
          "modules": {
            "A1-A3": {
              "value": 0.0184,
              "raw": "0.0184",
              "status": "declared",
              "provenance": {
                "page": 15,
                "section": "",
                "table": "",
                "module": "A1-A3",
                "unit_raw": "kg CO2 eq"
              }
            },
            "A4": {
              "value": 9.54e-07,
              "raw": "9.54E-7",
              "status": "declared",
              "provenance": {
                "page": 15,
                "section": "",
                "table": "",
                "module": "A4",
                "unit_raw": "kg CO2 eq"
              }
            },
            "A5": {
              "value": 0.000263,
              "raw": "0.000263",
              "status": "declared",
              "provenance": {
                "page": 15,
                "section": "",
                "table": "",
                "module": "A5",
                "unit_raw": "kg CO2 eq"
              }
            },
            "C1": {
              "value": 2.27e-05,
              "raw": "0.0000227",
              "status": "declared",
              "provenance": {
                "page": 15,
                "section": "",
                "table": "",
                "module": "C1",
                "unit_raw": "kg CO2 eq"
              }
            },
            "C2": {
              "value": 1.86e-06,
              "raw": "1.86E-6",
              "status": "declared",
              "provenance": {
                "page": 15,
                "section": "",
                "table": "",
                "module": "C2",
                "unit_raw": "kg CO2 eq"
              }
            },
            "C3": {
              "value": 3.5e-06,
              "raw": "3.50E-6",
              "status": "declared",
              "provenance": {
                "page": 15,
                "section": "",
                "table": "",
                "module": "C3",
                "unit_raw": "kg CO2 eq"
              }
            },
            "C4": {
              "value": 6.26e-05,
              "raw": "0.0000626",
              "status": "declared",
              "provenance": {
                "page": 15,
                "section": "",
                "table": "",
                "module": "C4",
                "unit_raw": "kg CO2 eq"
              }
            },
            "D": {
              "value": -0.0139,
              "raw": "-0.0139",
              "status": "declared",
              "provenance": {
                "page": 15,
                "section": "",
                "table": "",
                "module": "D",
                "unit_raw": "kg CO2 eq"
              }
            }
          }
        },
        "GWP_GHG": {
          "unit_raw": "kg CO2 eq",
          "unit_normalised": "kg CO2e",
          "header_modules": [
            "A1-A3",
            "A4",
            "A5",
            "C1",
            "C2",
            "C3",
            "C4",
            "D"
          ],
          "modules": {
            "A1-A3": {
              "value": 105.0,
              "raw": "105",
              "status": "declared",
              "provenance": {
                "page": 16,
                "section": "",
                "table": "",
                "module": "A1-A3",
                "unit_raw": "kg CO2 eq"
              }
            },
            "A4": {
              "value": 2.05,
              "raw": "2.05",
              "status": "declared",
              "provenance": {
                "page": 16,
                "section": "",
                "table": "",
                "module": "A4",
                "unit_raw": "kg CO2 eq"
              }
            },
            "A5": {
              "value": 8.81,
              "raw": "8.81",
              "status": "declared",
              "provenance": {
                "page": 16,
                "section": "",
                "table": "",
                "module": "A5",
                "unit_raw": "kg CO2 eq"
              }
            },
            "C1": {
              "value": 0.532,
              "raw": "0.532",
              "status": "declared",
              "provenance": {
                "page": 16,
                "section": "",
                "table": "",
                "module": "C1",
                "unit_raw": "kg CO2 eq"
              }
            },
            "C2": {
              "value": 3.99,
              "raw": "3.99",
              "status": "declared",
              "provenance": {
                "page": 16,
                "section": "",
                "table": "",
                "module": "C2",
                "unit_raw": "kg CO2 eq"
              }
            },
            "C3": {
              "value": 7.61,
              "raw": "7.61",
              "status": "declared",
              "provenance": {
                "page": 16,
                "section": "",
                "table": "",
                "module": "C3",
                "unit_raw": "kg CO2 eq"
              }
            },
            "C4": {
              "value": 1.28,
              "raw": "1.28",
              "status": "declared",
              "provenance": {
                "page": 16,
                "section": "",
                "table": "",
                "module": "C4",
                "unit_raw": "kg CO2 eq"
              }
            },
            "D": {
              "value": -15.7,
              "raw": "-15.7",
              "status": "declared",
              "provenance": {
                "page": 16,
                "section": "",
                "table": "",
                "module": "D",
                "unit_raw": "kg CO2 eq"
              }
            }
          }
        }
      }
    }
  ],
  "system_boundary": {
    "A1": "declared",
    "A2": "declared",
    "A3": "declared",
    "A1-A3": "declared",
    "A4": "declared",
    "A5": "declared",
    "B1": "not_declared",
    "B2": "not_declared",
    "B3": "not_declared",
    "B4": "not_declared",
    "B5": "not_declared",
    "B6": "not_declared",
    "B7": "not_declared",
    "C1": "declared",
    "C2": "declared",
    "C3": "declared",
    "C4": "declared",
    "D": "declared"
  },
  "comparability_notes": [
    "Cradle-to-gate (A1-A3) with options A4-A5, full C1-C4 and module D declared; use stage B1-B7 not declared (ND).",
    "C4 = 1.28 kg CO2e is a positive declared value here (unlike the QLD Holcim EPDs where C4 GWP prints 0).",
    "PCR version differs from the other Holcim files: this EPD uses PCR 2019:14 v1.3.4 (2024-04-30) + c-PCR-003 2024-04-30, whereas the SEQ/Brisbane files use PCR v2.0.1 (2025). Only compare EPDs on the same PCR first-digit version.",
    "Strength declared at 56 days (S32@56D), a later age than the typical 28-day basis — relevant when comparing strength-normalised carbon.",
    "GWP-GHG (AR5) row on page 16 (A1-A3=110, D=-15.2) is a separate AR5-based indicator, not an error vs GWP-Total (105).",
    "Declared unit 1 m3; product mass 2,400 kg/m3."
  ],
  "extraction_meta": {
    "method": "deterministic coordinate/order-bound table parse; contextual fields agent-verified",
    "numbers_validated": "cross_validate.py (raw string present on cited page)",
    "verified_by": "epd-context-agent (opus)",
    "checked_by": null,
    "confidence": "high",
    "warnings": [
      "Cell conflict across pages: GWP_GHG.A1-A3: '105' vs '110'",
      "Cell conflict across pages: GWP_GHG.A4: '2.05' vs '2.02'",
      "Cell conflict across pages: GWP_GHG.A5: '8.81' vs '8.65'",
      "Cell conflict across pages: GWP_GHG.C1: '0.532' vs '0.521'",
      "Cell conflict across pages: GWP_GHG.C2: '3.99' vs '3.95'",
      "Cell conflict across pages: GWP_GHG.C3: '7.61' vs '7.56'",
      "Cell conflict across pages: GWP_GHG.C4: '1.28' vs '1.25'",
      "Cell conflict across pages: GWP_GHG.D: '-15.7' vs '-15.2'",
      "Candidate extraction_meta 'cell conflicts' for GWP_GHG (e.g. A1-A3 '105' vs '110') compare the GWP-GHG row against the GWP-GHG (AR5) row on page 16 — different indicators, not a data error. GWP-Total values on page 15 confirmed correct."
    ],
    "needs_review": []
  }
}