{
  "schema_version": "1.0",
  "epd": {
    "id": "EPD-IES-23043",
    "source_pdf": "epd-ies-0023043-s32mpa-greencrete-70.pdf",
    "pages": 16,
    "program_operator": "The international EPD® system, www.environdec.com",
    "pcr": "2019:14 Construction Products, Version 1.3.4, 2024-04-",
    "reference_standard": null,
    "en15804_version": null,
    "characterisation": "EF 3.1",
    "published": null,
    "valid_until": "2025-06-20",
    "provenance": {
      "program_operator": {
        "page": 1,
        "snippet": "Programme operator: The international EPD® system, www.environdec.com"
      },
      "pcr": {
        "page": 2,
        "snippet": "PCR 2019:14 Construction Products, Version 1.3.4, 2024-04-"
      },
      "published": null,
      "valid_until": {
        "page": 2,
        "snippet": "valid until 2025-06-20"
      }
    }
  },
  "products": [
    {
      "name": "Premix Concrete – S32MPa GreenCrete 70",
      "manufacturer": "Piave Premix Concrete Pty Ltd",
      "concrete_type": null,
      "compressive_strength": {
        "value_mpa": 32,
        "class": null,
        "at_days": null,
        "raw": null,
        "status": "found",
        "provenance": {
          "page": 1,
          "snippet": "32MPA"
        }
      },
      "manufacturing_location": {
        "site": "262 Salmon Street, Port Melbourne VIC 3207",
        "city": "Port Melbourne",
        "region": "Victoria",
        "country": "AU",
        "raw": "262 Salmon Street Port Melbourne VIC 3207",
        "provenance": {
          "page": 2,
          "snippet": "Owner: Piave Premix Concrete Pty Ltd, 262 Salmon Street Port Melbourne VIC 3207"
        }
      },
      "declared_unit": {
        "amount": 1,
        "unit": "m3",
        "description": "1m3 of Premix Concrete supplied to the",
        "mass_kg": 2373.0,
        "provenance": {
          "page": 8,
          "snippet": "Declared unit | 1m3 of Premix Concrete supplied to the"
        }
      },
      "indicators": {
        "GWP_total": {
          "unit_raw": "kg CO2 eq",
          "unit_normalised": "kg CO2e",
          "header_modules": [
            "A1-A3",
            "C1",
            "C2",
            "C3",
            "C4",
            "D"
          ],
          "modules": {
            "A1-A3": {
              "value": 134.0,
              "raw": "1.34E+02",
              "status": "declared",
              "provenance": {
                "page": 11,
                "section": "CORE ENVIRONMENTAL IMPACT INDICATORS – EN 15804+A2, PEF",
                "table": "CORE ENVIRONMENTAL IMPACT INDICATORS – EN 15804+A2, PEF",
                "module": "A1-A3",
                "unit_raw": "kg CO2 eq"
              }
            },
            "C1": {
              "value": 5.67,
              "raw": "5.67E+00",
              "status": "declared",
              "provenance": {
                "page": 11,
                "section": "CORE ENVIRONMENTAL IMPACT INDICATORS – EN 15804+A2, PEF",
                "table": "CORE ENVIRONMENTAL IMPACT INDICATORS – EN 15804+A2, PEF",
                "module": "C1",
                "unit_raw": "kg CO2 eq"
              }
            },
            "C2": {
              "value": 21.6,
              "raw": "2.16E+01",
              "status": "declared",
              "provenance": {
                "page": 11,
                "section": "CORE ENVIRONMENTAL IMPACT INDICATORS – EN 15804+A2, PEF",
                "table": "CORE ENVIRONMENTAL IMPACT INDICATORS – EN 15804+A2, PEF",
                "module": "C2",
                "unit_raw": "kg CO2 eq"
              }
            },
            "C3": {
              "value": 12.5,
              "raw": "1.25E+01",
              "status": "declared",
              "provenance": {
                "page": 11,
                "section": "CORE ENVIRONMENTAL IMPACT INDICATORS – EN 15804+A2, PEF",
                "table": "CORE ENVIRONMENTAL IMPACT INDICATORS – EN 15804+A2, PEF",
                "module": "C3",
                "unit_raw": "kg CO2 eq"
              }
            },
            "C4": {
              "value": 2.29,
              "raw": "2.29E+00",
              "status": "declared",
              "provenance": {
                "page": 11,
                "section": "CORE ENVIRONMENTAL IMPACT INDICATORS – EN 15804+A2, PEF",
                "table": "CORE ENVIRONMENTAL IMPACT INDICATORS – EN 15804+A2, PEF",
                "module": "C4",
                "unit_raw": "kg CO2 eq"
              }
            },
            "D": {
              "value": -1.61,
              "raw": "‐1.61E+00",
              "status": "declared",
              "provenance": {
                "page": 11,
                "section": "CORE ENVIRONMENTAL IMPACT INDICATORS – EN 15804+A2, PEF",
                "table": "CORE ENVIRONMENTAL IMPACT INDICATORS – EN 15804+A2, PEF",
                "module": "D",
                "unit_raw": "kg CO2 eq"
              }
            }
          }
        },
        "GWP_fossil": {
          "unit_raw": "kg CO2 eq",
          "unit_normalised": "kg CO2e",
          "header_modules": [
            "A1-A3",
            "C1",
            "C2",
            "C3",
            "C4",
            "D"
          ],
          "modules": {
            "A1-A3": {
              "value": 134.0,
              "raw": "1.34E+02",
              "status": "declared",
              "provenance": {
                "page": 11,
                "section": "CORE ENVIRONMENTAL IMPACT INDICATORS – EN 15804+A2, PEF",
                "table": "CORE ENVIRONMENTAL IMPACT INDICATORS – EN 15804+A2, PEF",
                "module": "A1-A3",
                "unit_raw": "kg CO2 eq"
              }
            },
            "C1": {
              "value": 5.67,
              "raw": "5.67E+00",
              "status": "declared",
              "provenance": {
                "page": 11,
                "section": "CORE ENVIRONMENTAL IMPACT INDICATORS – EN 15804+A2, PEF",
                "table": "CORE ENVIRONMENTAL IMPACT INDICATORS – EN 15804+A2, PEF",
                "module": "C1",
                "unit_raw": "kg CO2 eq"
              }
            },
            "C2": {
              "value": 21.6,
              "raw": "2.16E+01",
              "status": "declared",
              "provenance": {
                "page": 11,
                "section": "CORE ENVIRONMENTAL IMPACT INDICATORS – EN 15804+A2, PEF",
                "table": "CORE ENVIRONMENTAL IMPACT INDICATORS – EN 15804+A2, PEF",
                "module": "C2",
                "unit_raw": "kg CO2 eq"
              }
            },
            "C3": {
              "value": 12.5,
              "raw": "1.25E+01",
              "status": "declared",
              "provenance": {
                "page": 11,
                "section": "CORE ENVIRONMENTAL IMPACT INDICATORS – EN 15804+A2, PEF",
                "table": "CORE ENVIRONMENTAL IMPACT INDICATORS – EN 15804+A2, PEF",
                "module": "C3",
                "unit_raw": "kg CO2 eq"
              }
            },
            "C4": {
              "value": 2.29,
              "raw": "2.29E+00",
              "status": "declared",
              "provenance": {
                "page": 11,
                "section": "CORE ENVIRONMENTAL IMPACT INDICATORS – EN 15804+A2, PEF",
                "table": "CORE ENVIRONMENTAL IMPACT INDICATORS – EN 15804+A2, PEF",
                "module": "C4",
                "unit_raw": "kg CO2 eq"
              }
            },
            "D": {
              "value": -1.61,
              "raw": "‐1.61E+00",
              "status": "declared",
              "provenance": {
                "page": 11,
                "section": "CORE ENVIRONMENTAL IMPACT INDICATORS – EN 15804+A2, PEF",
                "table": "CORE ENVIRONMENTAL IMPACT INDICATORS – EN 15804+A2, PEF",
                "module": "D",
                "unit_raw": "kg CO2 eq"
              }
            }
          }
        },
        "GWP_biogenic": {
          "unit_raw": "kg CO2 eq",
          "unit_normalised": "kg CO2e",
          "header_modules": [
            "A1-A3",
            "C1",
            "C2",
            "C3",
            "C4",
            "D"
          ],
          "modules": {
            "A1-A3": {
              "value": 0.0,
              "raw": "0.00E+00",
              "status": "declared_zero",
              "provenance": {
                "page": 11,
                "section": "CORE ENVIRONMENTAL IMPACT INDICATORS – EN 15804+A2, PEF",
                "table": "CORE ENVIRONMENTAL IMPACT INDICATORS – EN 15804+A2, PEF",
                "module": "A1-A3",
                "unit_raw": "kg CO2 eq"
              }
            },
            "C1": {
              "value": 0.0,
              "raw": "0.00E+00",
              "status": "declared_zero",
              "provenance": {
                "page": 11,
                "section": "CORE ENVIRONMENTAL IMPACT INDICATORS – EN 15804+A2, PEF",
                "table": "CORE ENVIRONMENTAL IMPACT INDICATORS – EN 15804+A2, PEF",
                "module": "C1",
                "unit_raw": "kg CO2 eq"
              }
            },
            "C2": {
              "value": 4.34e-19,
              "raw": "4.34E‐19",
              "status": "declared",
              "provenance": {
                "page": 11,
                "section": "CORE ENVIRONMENTAL IMPACT INDICATORS – EN 15804+A2, PEF",
                "table": "CORE ENVIRONMENTAL IMPACT INDICATORS – EN 15804+A2, PEF",
                "module": "C2",
                "unit_raw": "kg CO2 eq"
              }
            },
            "C3": {
              "value": 0.0,
              "raw": "0.00E+00",
              "status": "declared_zero",
              "provenance": {
                "page": 11,
                "section": "CORE ENVIRONMENTAL IMPACT INDICATORS – EN 15804+A2, PEF",
                "table": "CORE ENVIRONMENTAL IMPACT INDICATORS – EN 15804+A2, PEF",
                "module": "C3",
                "unit_raw": "kg CO2 eq"
              }
            },
            "C4": {
              "value": 0.0,
              "raw": "0.00E+00",
              "status": "declared_zero",
              "provenance": {
                "page": 11,
                "section": "CORE ENVIRONMENTAL IMPACT INDICATORS – EN 15804+A2, PEF",
                "table": "CORE ENVIRONMENTAL IMPACT INDICATORS – EN 15804+A2, PEF",
                "module": "C4",
                "unit_raw": "kg CO2 eq"
              }
            },
            "D": {
              "value": 0.0,
              "raw": "0.00E+00",
              "status": "declared_zero",
              "provenance": {
                "page": 11,
                "section": "CORE ENVIRONMENTAL IMPACT INDICATORS – EN 15804+A2, PEF",
                "table": "CORE ENVIRONMENTAL IMPACT INDICATORS – EN 15804+A2, PEF",
                "module": "D",
                "unit_raw": "kg CO2 eq"
              }
            }
          }
        },
        "GWP_luluc": {
          "unit_raw": "kg CO2 eq",
          "unit_normalised": "kg CO2e",
          "header_modules": [
            "A1-A3",
            "C1",
            "C2",
            "C3",
            "C4",
            "D"
          ],
          "modules": {
            "A1-A3": {
              "value": 0.0228,
              "raw": "2.28E‐02",
              "status": "declared",
              "provenance": {
                "page": 11,
                "section": "CORE ENVIRONMENTAL IMPACT INDICATORS – EN 15804+A2, PEF",
                "table": "CORE ENVIRONMENTAL IMPACT INDICATORS – EN 15804+A2, PEF",
                "module": "A1-A3",
                "unit_raw": "kg CO2 eq"
              }
            },
            "C1": {
              "value": 0.000565,
              "raw": "5.65E‐04",
              "status": "declared",
              "provenance": {
                "page": 11,
                "section": "CORE ENVIRONMENTAL IMPACT INDICATORS – EN 15804+A2, PEF",
                "table": "CORE ENVIRONMENTAL IMPACT INDICATORS – EN 15804+A2, PEF",
                "module": "C1",
                "unit_raw": "kg CO2 eq"
              }
            },
            "C2": {
              "value": 0.00769,
              "raw": "7.69E‐03",
              "status": "declared",
              "provenance": {
                "page": 11,
                "section": "CORE ENVIRONMENTAL IMPACT INDICATORS – EN 15804+A2, PEF",
                "table": "CORE ENVIRONMENTAL IMPACT INDICATORS – EN 15804+A2, PEF",
                "module": "C2",
                "unit_raw": "kg CO2 eq"
              }
            },
            "C3": {
              "value": 0.00128,
              "raw": "1.28E‐03",
              "status": "declared",
              "provenance": {
                "page": 11,
                "section": "CORE ENVIRONMENTAL IMPACT INDICATORS – EN 15804+A2, PEF",
                "table": "CORE ENVIRONMENTAL IMPACT INDICATORS – EN 15804+A2, PEF",
                "module": "C3",
                "unit_raw": "kg CO2 eq"
              }
            },
            "C4": {
              "value": 0.00131,
              "raw": "1.31E‐03",
              "status": "declared",
              "provenance": {
                "page": 11,
                "section": "CORE ENVIRONMENTAL IMPACT INDICATORS – EN 15804+A2, PEF",
                "table": "CORE ENVIRONMENTAL IMPACT INDICATORS – EN 15804+A2, PEF",
                "module": "C4",
                "unit_raw": "kg CO2 eq"
              }
            },
            "D": {
              "value": -0.000172,
              "raw": "‐1.72E‐04",
              "status": "declared",
              "provenance": {
                "page": 11,
                "section": "CORE ENVIRONMENTAL IMPACT INDICATORS – EN 15804+A2, PEF",
                "table": "CORE ENVIRONMENTAL IMPACT INDICATORS – EN 15804+A2, PEF",
                "module": "D",
                "unit_raw": "kg CO2 eq"
              }
            }
          }
        },
        "GWP_GHG": {
          "unit_raw": "kg CO2 eq",
          "unit_normalised": "kg CO2e",
          "header_modules": [
            "A1-A3",
            "C1",
            "C2",
            "C3",
            "C4",
            "D"
          ],
          "modules": {
            "A1-A3": {
              "value": 134.0,
              "raw": "1.34E+02",
              "status": "declared",
              "provenance": {
                "page": 13,
                "section": "ENVIRONMENTAL INFORMATION DESCRIBING WASTE CATEGORIES",
                "table": "ENVIRONMENTAL INFORMATION DESCRIBING WASTE CATEGORIES",
                "module": "A1-A3",
                "unit_raw": "kg CO2 eq"
              }
            },
            "C1": {
              "value": 5.67,
              "raw": "5.67E+00",
              "status": "declared",
              "provenance": {
                "page": 13,
                "section": "ENVIRONMENTAL INFORMATION DESCRIBING WASTE CATEGORIES",
                "table": "ENVIRONMENTAL INFORMATION DESCRIBING WASTE CATEGORIES",
                "module": "C1",
                "unit_raw": "kg CO2 eq"
              }
            },
            "C2": {
              "value": 21.6,
              "raw": "2.16E+01",
              "status": "declared",
              "provenance": {
                "page": 13,
                "section": "ENVIRONMENTAL INFORMATION DESCRIBING WASTE CATEGORIES",
                "table": "ENVIRONMENTAL INFORMATION DESCRIBING WASTE CATEGORIES",
                "module": "C2",
                "unit_raw": "kg CO2 eq"
              }
            },
            "C3": {
              "value": 12.5,
              "raw": "1.25E+01",
              "status": "declared",
              "provenance": {
                "page": 13,
                "section": "ENVIRONMENTAL INFORMATION DESCRIBING WASTE CATEGORIES",
                "table": "ENVIRONMENTAL INFORMATION DESCRIBING WASTE CATEGORIES",
                "module": "C3",
                "unit_raw": "kg CO2 eq"
              }
            },
            "C4": {
              "value": 2.29,
              "raw": "2.29E+00",
              "status": "declared",
              "provenance": {
                "page": 13,
                "section": "ENVIRONMENTAL INFORMATION DESCRIBING WASTE CATEGORIES",
                "table": "ENVIRONMENTAL INFORMATION DESCRIBING WASTE CATEGORIES",
                "module": "C4",
                "unit_raw": "kg CO2 eq"
              }
            },
            "D": {
              "value": -1.61,
              "raw": "‐1.61E+00",
              "status": "declared",
              "provenance": {
                "page": 13,
                "section": "ENVIRONMENTAL INFORMATION DESCRIBING WASTE CATEGORIES",
                "table": "ENVIRONMENTAL INFORMATION DESCRIBING WASTE CATEGORIES",
                "module": "D",
                "unit_raw": "kg CO2 eq"
              }
            }
          }
        }
      }
    }
  ],
  "system_boundary": {
    "A1": "not_declared",
    "A2": "not_declared",
    "A3": "not_declared",
    "A1-A3": "declared",
    "A4": "not_declared",
    "A5": "not_declared",
    "B1": "not_declared",
    "B2": "not_declared",
    "B3": "not_declared",
    "B4": "not_declared",
    "B5": "not_declared",
    "B6": "not_declared",
    "B7": "not_declared",
    "C1": "declared",
    "C2": "declared",
    "C3": "declared",
    "C4": "declared",
    "D": "declared"
  },
  "comparability_notes": [],
  "extraction_meta": {
    "method": "deterministic coordinate/order-bound table parse; contextual fields agent-verified",
    "numbers_validated": "cross_validate.py (raw string present on cited page)",
    "verified_by": "main-agent source-read fix",
    "checked_by": null,
    "confidence": "high",
    "warnings": [],
    "needs_review": []
  }
}