{
  "schema_version": "1.0",
  "epd": {
    "id": "EPD-IES-0014769:001",
    "source_pdf": "EPD-IES-0014769_P252080.pdf",
    "pages": 28,
    "program_operator": "EPD International AB",
    "pcr": "CEN standard EN 15804:A2 (PCR 2019:14 Construction Products, Version 1.3.4) served as the core PCR; Environdec c-PCR-003 Concrete, concrete elements (EN 16757:2023) served as sub-PCR.",
    "reference_standard": "EN 15804:A2 (in accordance with ISO 14025, EN 16757, Environdec c-PCR-003)",
    "en15804_version": "A2",
    "characterisation": "EF 3.1",
    "published": "2024-08-26",
    "valid_until": "2029-08-26",
    "provenance": {
      "program_operator": {
        "page": 1,
        "snippet": "Programme Operator: EPD International AB"
      },
      "pcr": {
        "page": 24,
        "snippet": "Product Category Rules | CEN standard EN 15804:A2 (PCR 2019:14 Construction Products, Version  1.3.4) served as the core PCR."
      },
      "published": null,
      "valid_until": null
    },
    "page_labels": null
  },
  "products": [
    {
      "name": "P252080 (Hutchinson Builders - Aliro Warehouse)",
      "manufacturer": "Hanson Construction Materials Pty Ltd",
      "concrete_type": "Ready-mix concrete",
      "compressive_strength": {
        "value_mpa": 25,
        "class": null,
        "at_days": null,
        "raw": "Compressive Strength 25",
        "status": "found",
        "provenance": {
          "page": 20,
          "snippet": "Product Identification P252080 ... Compressive Strength 25 Density 2480 kg/m³"
        }
      },
      "manufacturing_location": {
        "site": "Brisbane",
        "city": "Brisbane",
        "region": "Queensland",
        "country": "AU",
        "raw": "Production Site(S) Brisbane",
        "provenance": {
          "page": 20,
          "snippet": "Production Site(S) Brisbane"
        },
        "note": "Geographical Scope 'Queensland - Brisbane' also stated on page 1 and page 24."
      },
      "declared_unit": {
        "amount": 1,
        "unit": "m3",
        "description": "Declared Unit is 1m3 of Concrete",
        "mass_kg": 2480,
        "provenance": {
          "page": 20,
          "snippet": "Declared Unit 1 m3 ... Density 2480 kg/m³"
        }
      },
      "indicators": {
        "GWP_GHG": {
          "unit_raw": "kg CO₂e",
          "unit_normalised": "kg CO2e",
          "header_modules": [
            "A1-A3",
            "A4",
            "A5",
            "B1",
            "B2",
            "B3",
            "B4",
            "B5",
            "B6",
            "B7",
            "C1",
            "C2",
            "C3",
            "C4",
            "D"
          ],
          "modules": {
            "A1-A3": {
              "value": 127.0,
              "raw": "1.27E+02",
              "status": "declared",
              "provenance": {
                "page": 21,
                "section": "",
                "table": "",
                "module": "A1-A3",
                "unit_raw": "kg CO₂e"
              }
            },
            "A4": {
              "value": 2.45,
              "raw": "2.45E+00",
              "status": "declared",
              "provenance": {
                "page": 21,
                "section": "",
                "table": "",
                "module": "A4",
                "unit_raw": "kg CO₂e"
              }
            },
            "A5": {
              "value": 9.95,
              "raw": "9.95E+00",
              "status": "declared",
              "provenance": {
                "page": 21,
                "section": "",
                "table": "",
                "module": "A5",
                "unit_raw": "kg CO₂e"
              }
            },
            "B1": {
              "value": -2.65,
              "raw": "-2.65E+00",
              "status": "declared",
              "provenance": {
                "page": 21,
                "section": "",
                "table": "",
                "module": "B1",
                "unit_raw": "kg CO₂e"
              }
            },
            "B2": {
              "value": 0.0,
              "raw": "0.00E+00",
              "status": "declared_zero",
              "provenance": {
                "page": 21,
                "section": "",
                "table": "",
                "module": "B2",
                "unit_raw": "kg CO₂e"
              }
            },
            "B3": {
              "value": 0.0,
              "raw": "0.00E+00",
              "status": "declared_zero",
              "provenance": {
                "page": 21,
                "section": "",
                "table": "",
                "module": "B3",
                "unit_raw": "kg CO₂e"
              }
            },
            "B4": {
              "value": 0.0,
              "raw": "0.00E+00",
              "status": "declared_zero",
              "provenance": {
                "page": 21,
                "section": "",
                "table": "",
                "module": "B4",
                "unit_raw": "kg CO₂e"
              }
            },
            "B5": {
              "value": 0.0,
              "raw": "0.00E+00",
              "status": "declared_zero",
              "provenance": {
                "page": 21,
                "section": "",
                "table": "",
                "module": "B5",
                "unit_raw": "kg CO₂e"
              }
            },
            "B6": {
              "value": 0.0,
              "raw": "0.00E+00",
              "status": "declared_zero",
              "provenance": {
                "page": 21,
                "section": "",
                "table": "",
                "module": "B6",
                "unit_raw": "kg CO₂e"
              }
            },
            "B7": {
              "value": 0.0,
              "raw": "0.00E+00",
              "status": "declared_zero",
              "provenance": {
                "page": 21,
                "section": "",
                "table": "",
                "module": "B7",
                "unit_raw": "kg CO₂e"
              }
            },
            "C1": {
              "value": 8.99,
              "raw": "8.99E+00",
              "status": "declared",
              "provenance": {
                "page": 21,
                "section": "",
                "table": "",
                "module": "C1",
                "unit_raw": "kg CO₂e"
              }
            },
            "C2": {
              "value": 8.85,
              "raw": "8.85E+00",
              "status": "declared",
              "provenance": {
                "page": 21,
                "section": "",
                "table": "",
                "module": "C2",
                "unit_raw": "kg CO₂e"
              }
            },
            "C3": {
              "value": 5.24,
              "raw": "5.24E+00",
              "status": "declared",
              "provenance": {
                "page": 21,
                "section": "",
                "table": "",
                "module": "C3",
                "unit_raw": "kg CO₂e"
              }
            },
            "C4": {
              "value": 2.79,
              "raw": "2.79E+00",
              "status": "declared",
              "provenance": {
                "page": 21,
                "section": "",
                "table": "",
                "module": "C4",
                "unit_raw": "kg CO₂e"
              }
            },
            "D": {
              "value": 6.14,
              "raw": "6.14E+00",
              "status": "declared",
              "provenance": {
                "page": 21,
                "section": "",
                "table": "",
                "module": "D",
                "unit_raw": "kg CO₂e"
              }
            }
          }
        },
        "GWP_total": {
          "unit_raw": "kg CO₂e",
          "unit_normalised": "kg CO2e",
          "header_modules": [
            "A1-A3",
            "A4",
            "A5",
            "B1",
            "B2",
            "B3",
            "B4",
            "B5",
            "B6",
            "B7",
            "C1",
            "C2",
            "C3",
            "C4",
            "D"
          ],
          "modules": {
            "A1-A3": {
              "value": 127.0,
              "raw": "1.27E+02",
              "status": "declared",
              "provenance": {
                "page": 21,
                "section": "",
                "table": "",
                "module": "A1-A3",
                "unit_raw": "kg CO₂e"
              }
            },
            "A4": {
              "value": 2.45,
              "raw": "2.45E+00",
              "status": "declared",
              "provenance": {
                "page": 21,
                "section": "",
                "table": "",
                "module": "A4",
                "unit_raw": "kg CO₂e"
              }
            },
            "A5": {
              "value": 9.95,
              "raw": "9.95E+00",
              "status": "declared",
              "provenance": {
                "page": 21,
                "section": "",
                "table": "",
                "module": "A5",
                "unit_raw": "kg CO₂e"
              }
            },
            "B1": {
              "value": -2.65,
              "raw": "-2.65E+00",
              "status": "declared",
              "provenance": {
                "page": 21,
                "section": "",
                "table": "",
                "module": "B1",
                "unit_raw": "kg CO₂e"
              }
            },
            "B2": {
              "value": 0.0,
              "raw": "0.00E+00",
              "status": "declared_zero",
              "provenance": {
                "page": 21,
                "section": "",
                "table": "",
                "module": "B2",
                "unit_raw": "kg CO₂e"
              }
            },
            "B3": {
              "value": 0.0,
              "raw": "0.00E+00",
              "status": "declared_zero",
              "provenance": {
                "page": 21,
                "section": "",
                "table": "",
                "module": "B3",
                "unit_raw": "kg CO₂e"
              }
            },
            "B4": {
              "value": 0.0,
              "raw": "0.00E+00",
              "status": "declared_zero",
              "provenance": {
                "page": 21,
                "section": "",
                "table": "",
                "module": "B4",
                "unit_raw": "kg CO₂e"
              }
            },
            "B5": {
              "value": 0.0,
              "raw": "0.00E+00",
              "status": "declared_zero",
              "provenance": {
                "page": 21,
                "section": "",
                "table": "",
                "module": "B5",
                "unit_raw": "kg CO₂e"
              }
            },
            "B6": {
              "value": 0.0,
              "raw": "0.00E+00",
              "status": "declared_zero",
              "provenance": {
                "page": 21,
                "section": "",
                "table": "",
                "module": "B6",
                "unit_raw": "kg CO₂e"
              }
            },
            "B7": {
              "value": 0.0,
              "raw": "0.00E+00",
              "status": "declared_zero",
              "provenance": {
                "page": 21,
                "section": "",
                "table": "",
                "module": "B7",
                "unit_raw": "kg CO₂e"
              }
            },
            "C1": {
              "value": 8.99,
              "raw": "8.99E+00",
              "status": "declared",
              "provenance": {
                "page": 21,
                "section": "",
                "table": "",
                "module": "C1",
                "unit_raw": "kg CO₂e"
              }
            },
            "C2": {
              "value": 8.85,
              "raw": "8.85E+00",
              "status": "declared",
              "provenance": {
                "page": 21,
                "section": "",
                "table": "",
                "module": "C2",
                "unit_raw": "kg CO₂e"
              }
            },
            "C3": {
              "value": 5.24,
              "raw": "5.24E+00",
              "status": "declared",
              "provenance": {
                "page": 21,
                "section": "",
                "table": "",
                "module": "C3",
                "unit_raw": "kg CO₂e"
              }
            },
            "C4": {
              "value": 2.79,
              "raw": "2.79E+00",
              "status": "declared",
              "provenance": {
                "page": 21,
                "section": "",
                "table": "",
                "module": "C4",
                "unit_raw": "kg CO₂e"
              }
            },
            "D": {
              "value": 6.14,
              "raw": "6.14E+00",
              "status": "declared",
              "provenance": {
                "page": 21,
                "section": "",
                "table": "",
                "module": "D",
                "unit_raw": "kg CO₂e"
              }
            }
          }
        },
        "GWP_fossil": {
          "unit_raw": "kg CO₂e",
          "unit_normalised": "kg CO2e",
          "header_modules": [
            "A1-A3",
            "A4",
            "A5",
            "B1",
            "B2",
            "B3",
            "B4",
            "B5",
            "B6",
            "B7",
            "C1",
            "C2",
            "C3",
            "C4",
            "D"
          ],
          "modules": {
            "A1-A3": {
              "value": 126.0,
              "raw": "1.26E+02",
              "status": "declared",
              "provenance": {
                "page": 21,
                "section": "",
                "table": "",
                "module": "A1-A3",
                "unit_raw": "kg CO₂e"
              }
            },
            "A4": {
              "value": 2.45,
              "raw": "2.45E+00",
              "status": "declared",
              "provenance": {
                "page": 21,
                "section": "",
                "table": "",
                "module": "A4",
                "unit_raw": "kg CO₂e"
              }
            },
            "A5": {
              "value": 9.94,
              "raw": "9.94E+00",
              "status": "declared",
              "provenance": {
                "page": 21,
                "section": "",
                "table": "",
                "module": "A5",
                "unit_raw": "kg CO₂e"
              }
            },
            "B1": {
              "value": -2.65,
              "raw": "-2.65E+00",
              "status": "declared",
              "provenance": {
                "page": 21,
                "section": "",
                "table": "",
                "module": "B1",
                "unit_raw": "kg CO₂e"
              }
            },
            "B2": {
              "value": 0.0,
              "raw": "0.00E+00",
              "status": "declared_zero",
              "provenance": {
                "page": 21,
                "section": "",
                "table": "",
                "module": "B2",
                "unit_raw": "kg CO₂e"
              }
            },
            "B3": {
              "value": 0.0,
              "raw": "0.00E+00",
              "status": "declared_zero",
              "provenance": {
                "page": 21,
                "section": "",
                "table": "",
                "module": "B3",
                "unit_raw": "kg CO₂e"
              }
            },
            "B4": {
              "value": 0.0,
              "raw": "0.00E+00",
              "status": "declared_zero",
              "provenance": {
                "page": 21,
                "section": "",
                "table": "",
                "module": "B4",
                "unit_raw": "kg CO₂e"
              }
            },
            "B5": {
              "value": 0.0,
              "raw": "0.00E+00",
              "status": "declared_zero",
              "provenance": {
                "page": 21,
                "section": "",
                "table": "",
                "module": "B5",
                "unit_raw": "kg CO₂e"
              }
            },
            "B6": {
              "value": 0.0,
              "raw": "0.00E+00",
              "status": "declared_zero",
              "provenance": {
                "page": 21,
                "section": "",
                "table": "",
                "module": "B6",
                "unit_raw": "kg CO₂e"
              }
            },
            "B7": {
              "value": 0.0,
              "raw": "0.00E+00",
              "status": "declared_zero",
              "provenance": {
                "page": 21,
                "section": "",
                "table": "",
                "module": "B7",
                "unit_raw": "kg CO₂e"
              }
            },
            "C1": {
              "value": 8.99,
              "raw": "8.99E+00",
              "status": "declared",
              "provenance": {
                "page": 21,
                "section": "",
                "table": "",
                "module": "C1",
                "unit_raw": "kg CO₂e"
              }
            },
            "C2": {
              "value": 8.84,
              "raw": "8.84E+00",
              "status": "declared",
              "provenance": {
                "page": 21,
                "section": "",
                "table": "",
                "module": "C2",
                "unit_raw": "kg CO₂e"
              }
            },
            "C3": {
              "value": 5.21,
              "raw": "5.21E+00",
              "status": "declared",
              "provenance": {
                "page": 21,
                "section": "",
                "table": "",
                "module": "C3",
                "unit_raw": "kg CO₂e"
              }
            },
            "C4": {
              "value": 2.79,
              "raw": "2.79E+00",
              "status": "declared",
              "provenance": {
                "page": 21,
                "section": "",
                "table": "",
                "module": "C4",
                "unit_raw": "kg CO₂e"
              }
            },
            "D": {
              "value": 6.11,
              "raw": "6.11E+00",
              "status": "declared",
              "provenance": {
                "page": 21,
                "section": "",
                "table": "",
                "module": "D",
                "unit_raw": "kg CO₂e"
              }
            }
          }
        },
        "GWP_biogenic": {
          "unit_raw": "kg CO₂e",
          "unit_normalised": "kg CO2e",
          "header_modules": [
            "A1-A3",
            "A4",
            "A5",
            "B1",
            "B2",
            "B3",
            "B4",
            "B5",
            "B6",
            "B7",
            "C1",
            "C2",
            "C3",
            "C4",
            "D"
          ],
          "modules": {
            "A1-A3": {
              "value": 0.0462,
              "raw": "4.62E-02",
              "status": "declared",
              "provenance": {
                "page": 21,
                "section": "",
                "table": "",
                "module": "A1-A3",
                "unit_raw": "kg CO₂e"
              }
            },
            "A4": {
              "value": 0.000959,
              "raw": "9.59E-04",
              "status": "declared",
              "provenance": {
                "page": 21,
                "section": "",
                "table": "",
                "module": "A4",
                "unit_raw": "kg CO₂e"
              }
            },
            "A5": {
              "value": 0.00435,
              "raw": "4.35E-03",
              "status": "declared",
              "provenance": {
                "page": 21,
                "section": "",
                "table": "",
                "module": "A5",
                "unit_raw": "kg CO₂e"
              }
            },
            "B1": {
              "value": 0.0,
              "raw": "0.00E+00",
              "status": "declared_zero",
              "provenance": {
                "page": 21,
                "section": "",
                "table": "",
                "module": "B1",
                "unit_raw": "kg CO₂e"
              }
            },
            "B2": {
              "value": 0.0,
              "raw": "0.00E+00",
              "status": "declared_zero",
              "provenance": {
                "page": 21,
                "section": "",
                "table": "",
                "module": "B2",
                "unit_raw": "kg CO₂e"
              }
            },
            "B3": {
              "value": 0.0,
              "raw": "0.00E+00",
              "status": "declared_zero",
              "provenance": {
                "page": 21,
                "section": "",
                "table": "",
                "module": "B3",
                "unit_raw": "kg CO₂e"
              }
            },
            "B4": {
              "value": 0.0,
              "raw": "0.00E+00",
              "status": "declared_zero",
              "provenance": {
                "page": 21,
                "section": "",
                "table": "",
                "module": "B4",
                "unit_raw": "kg CO₂e"
              }
            },
            "B5": {
              "value": 0.0,
              "raw": "0.00E+00",
              "status": "declared_zero",
              "provenance": {
                "page": 21,
                "section": "",
                "table": "",
                "module": "B5",
                "unit_raw": "kg CO₂e"
              }
            },
            "B6": {
              "value": 0.0,
              "raw": "0.00E+00",
              "status": "declared_zero",
              "provenance": {
                "page": 21,
                "section": "",
                "table": "",
                "module": "B6",
                "unit_raw": "kg CO₂e"
              }
            },
            "B7": {
              "value": 0.0,
              "raw": "0.00E+00",
              "status": "declared_zero",
              "provenance": {
                "page": 21,
                "section": "",
                "table": "",
                "module": "B7",
                "unit_raw": "kg CO₂e"
              }
            },
            "C1": {
              "value": 0.0016,
              "raw": "1.60E-03",
              "status": "declared",
              "provenance": {
                "page": 21,
                "section": "",
                "table": "",
                "module": "C1",
                "unit_raw": "kg CO₂e"
              }
            },
            "C2": {
              "value": 0.00632,
              "raw": "6.32E-03",
              "status": "declared",
              "provenance": {
                "page": 21,
                "section": "",
                "table": "",
                "module": "C2",
                "unit_raw": "kg CO₂e"
              }
            },
            "C3": {
              "value": 0.0189,
              "raw": "1.89E-02",
              "status": "declared",
              "provenance": {
                "page": 21,
                "section": "",
                "table": "",
                "module": "C3",
                "unit_raw": "kg CO₂e"
              }
            },
            "C4": {
              "value": 0.00184,
              "raw": "1.84E-03",
              "status": "declared",
              "provenance": {
                "page": 21,
                "section": "",
                "table": "",
                "module": "C4",
                "unit_raw": "kg CO₂e"
              }
            },
            "D": {
              "value": 0.0189,
              "raw": "1.89E-02",
              "status": "declared",
              "provenance": {
                "page": 21,
                "section": "",
                "table": "",
                "module": "D",
                "unit_raw": "kg CO₂e"
              }
            }
          }
        },
        "GWP_luluc": {
          "unit_raw": "kg CO₂e",
          "unit_normalised": "kg CO2e",
          "header_modules": [
            "A1-A3",
            "A4",
            "A5",
            "B1",
            "B2",
            "B3",
            "B4",
            "B5",
            "B6",
            "B7",
            "C1",
            "C2",
            "C3",
            "C4",
            "D"
          ],
          "modules": {
            "A1-A3": {
              "value": 0.0292,
              "raw": "2.92E-02",
              "status": "declared",
              "provenance": {
                "page": 21,
                "section": "",
                "table": "",
                "module": "A1-A3",
                "unit_raw": "kg CO₂e"
              }
            },
            "A4": {
              "value": 0.000829,
              "raw": "8.29E-04",
              "status": "declared",
              "provenance": {
                "page": 21,
                "section": "",
                "table": "",
                "module": "A4",
                "unit_raw": "kg CO₂e"
              }
            },
            "A5": {
              "value": 0.00331,
              "raw": "3.31E-03",
              "status": "declared",
              "provenance": {
                "page": 21,
                "section": "",
                "table": "",
                "module": "A5",
                "unit_raw": "kg CO₂e"
              }
            },
            "B1": {
              "value": 0.0,
              "raw": "0.00E+00",
              "status": "declared_zero",
              "provenance": {
                "page": 21,
                "section": "",
                "table": "",
                "module": "B1",
                "unit_raw": "kg CO₂e"
              }
            },
            "B2": {
              "value": 0.0,
              "raw": "0.00E+00",
              "status": "declared_zero",
              "provenance": {
                "page": 21,
                "section": "",
                "table": "",
                "module": "B2",
                "unit_raw": "kg CO₂e"
              }
            },
            "B3": {
              "value": 0.0,
              "raw": "0.00E+00",
              "status": "declared_zero",
              "provenance": {
                "page": 21,
                "section": "",
                "table": "",
                "module": "B3",
                "unit_raw": "kg CO₂e"
              }
            },
            "B4": {
              "value": 0.0,
              "raw": "0.00E+00",
              "status": "declared_zero",
              "provenance": {
                "page": 21,
                "section": "",
                "table": "",
                "module": "B4",
                "unit_raw": "kg CO₂e"
              }
            },
            "B5": {
              "value": 0.0,
              "raw": "0.00E+00",
              "status": "declared_zero",
              "provenance": {
                "page": 21,
                "section": "",
                "table": "",
                "module": "B5",
                "unit_raw": "kg CO₂e"
              }
            },
            "B6": {
              "value": 0.0,
              "raw": "0.00E+00",
              "status": "declared_zero",
              "provenance": {
                "page": 21,
                "section": "",
                "table": "",
                "module": "B6",
                "unit_raw": "kg CO₂e"
              }
            },
            "B7": {
              "value": 0.0,
              "raw": "0.00E+00",
              "status": "declared_zero",
              "provenance": {
                "page": 21,
                "section": "",
                "table": "",
                "module": "B7",
                "unit_raw": "kg CO₂e"
              }
            },
            "C1": {
              "value": 0.00113,
              "raw": "1.13E-03",
              "status": "declared",
              "provenance": {
                "page": 21,
                "section": "",
                "table": "",
                "module": "C1",
                "unit_raw": "kg CO₂e"
              }
            },
            "C2": {
              "value": 0.00514,
              "raw": "5.14E-03",
              "status": "declared",
              "provenance": {
                "page": 21,
                "section": "",
                "table": "",
                "module": "C2",
                "unit_raw": "kg CO₂e"
              }
            },
            "C3": {
              "value": 0.0144,
              "raw": "1.44E-02",
              "status": "declared",
              "provenance": {
                "page": 21,
                "section": "",
                "table": "",
                "module": "C3",
                "unit_raw": "kg CO₂e"
              }
            },
            "C4": {
              "value": 0.0015,
              "raw": "1.50E-03",
              "status": "declared",
              "provenance": {
                "page": 21,
                "section": "",
                "table": "",
                "module": "C4",
                "unit_raw": "kg CO₂e"
              }
            },
            "D": {
              "value": 0.0144,
              "raw": "1.44E-02",
              "status": "declared",
              "provenance": {
                "page": 21,
                "section": "",
                "table": "",
                "module": "D",
                "unit_raw": "kg CO₂e"
              }
            }
          }
        }
      }
    }
  ],
  "system_boundary": {
    "A1": "not_declared",
    "A2": "not_declared",
    "A3": "not_declared",
    "A1-A3": "declared",
    "A4": "declared",
    "A5": "declared",
    "B1": "declared",
    "B2": "declared_zero",
    "B3": "declared_zero",
    "B4": "declared_zero",
    "B5": "declared_zero",
    "B6": "declared_zero",
    "B7": "declared_zero",
    "C1": "declared",
    "C2": "declared",
    "C3": "declared",
    "C4": "declared",
    "D": "declared"
  },
  "comparability_notes": [
    "GCCA Industry EPD Tool for Cement and Concrete (v4.2), International version, used to model results (page 20).",
    "Full cradle-to-grave scope A1-A3 + A4 + A5 + B1-B7 + C1-C4 + D — all modules declared; no ND/NR modules.",
    "GWP reported as GWP-tot per the GCCA tool; GWP-GHG and GWP-tot are numerically identical in this EPD (page 21).",
    "Project-specific EPD (Hutchinson Builders - Aliro Warehouse project); values indicative of local material performance at time of publishing (page 18).",
    "EPDs from different programmes or that do not comply with EN 15804 may not be comparable (page 24)."
  ],
  "extraction_meta": {
    "method": "deterministic coordinate/order-bound table parse; contextual fields agent-verified",
    "numbers_validated": "cross_validate.py (raw string present on cited page)",
    "verified_by": "epd-context-agent (Opus 4.8)",
    "checked_by": null,
    "confidence": "high",
    "warnings": [
      "Candidate compressive_strength.value_mpa was 40 (class '[MPa]') — INCORRECT. Verified correct value is 25 MPa (pages 18 and 20). GWP numbers not affected; only the strength field was mis-bound in the candidate."
    ],
    "needs_review": []
  }
}