{
  "schema_version": "1.0",
  "epd": {
    "id": "EPD-IES-0029695:001",
    "source_pdf": "epd-australasia-com-wp-content-uploads-2025-05-epd-ies-0029695-001-holcim-qld-brisbane-ecopact-qe252m100-2026-04-15-1-pdf.pdf",
    "pages": 21,
    "program_operator": "EPD International AB (International EPD System); Regional Programme: EPD Australasia",
    "pcr": "PCR 2019:14 Construction Products, Version 2.0.1, 2025-06-05; c-PCR-003 Concrete and Concrete Elements, 2025-04-08",
    "reference_standard": "EN 15804:2012+A2:2019/AC:2021 (ISO 14025)",
    "en15804_version": "A2",
    "characterisation": "EF 3.1",
    "published": "2026-04-15",
    "valid_until": "2031-04-15",
    "provenance": {
      "program_operator": {
        "page": 1,
        "snippet": "Programme operator: EPD International AB"
      },
      "pcr": {
        "page": 2,
        "snippet": "Product category rules | PCR 2019:14 Construction Products, Version 2.0.1, 2025-06-05"
      },
      "published": null,
      "valid_until": {
        "page": 2,
        "snippet": "Valid Until\n15/4/2031"
      }
    }
  },
  "products": [
    {
      "name": "QLD - Brisbane - ECOPact - QE252M100 - S25/20/100 Ecopact Concrete - General use",
      "manufacturer": "Holcim (Australia) Pty Ltd",
      "concrete_type": "Ready-mix concrete",
      "compressive_strength": {
        "value_mpa": 25,
        "class": "S25/20/100",
        "at_days": 28,
        "raw": "Strength (MPa) 25 | Mix Code QE252M100 | S25/20/100 Ecopact Concrete",
        "status": "found",
        "provenance": {
          "page": 10,
          "snippet": "Strength (MPa) ... 25 QE252M100 2319 S25/20/100 Ecopact Concrete General use"
        }
      },
      "manufacturing_location": {
        "site": "Brisbane network of Holcim batching plants",
        "city": "Brisbane City (plus Acacia Ridge, Darra, Geebung, Wacol, Murarrie, etc.)",
        "region": "QLD",
        "country": "AU",
        "raw": "Production Sites: Brisbane City, Acacia Ridge, Beaudesert, Beenleigh, Boonah, Darra, Cleveland, Geebung, Narangba, Wacol, Murarrie, Caboolture, Brendale, Raceview.",
        "provenance": {
          "page": 10,
          "snippet": "Production Sites Brisbane City, Acacia Ridge, Beaudesert, Beenleigh, Boonah, Darra, Cleveland, Geebung, Narangba, Wacol, Murarrie, Caboolture, Brendale, Raceview."
        },
        "note": "Multi-plant Brisbane EPD. The page-6 'Address and Contact Information' (100 Miller St, North Sydney) is the corporate/EPD-owner HQ, not a production site."
      },
      "declared_unit": {
        "amount": 1,
        "unit": "m3",
        "description": "1 m3 of ready-mix concrete.",
        "mass_kg": 2319,
        "provenance": {
          "page": 6,
          "snippet": "Declared Unit 1 m3 of ready-mix concrete."
        }
      },
      "indicators": {
        "GWP_total": {
          "unit_raw": "kg CO2 eq",
          "unit_normalised": "kg CO2e",
          "header_modules": [
            "A1-A3",
            "A4",
            "A5",
            "C1",
            "C2",
            "C3",
            "C4",
            "D"
          ],
          "modules": {
            "A1-A3": {
              "value": 146.0,
              "raw": "146",
              "status": "declared",
              "provenance": {
                "page": 16,
                "section": "",
                "table": "",
                "module": "A1-A3",
                "unit_raw": "kg CO2 eq"
              }
            },
            "A4": {
              "value": 2.58,
              "raw": "2.58",
              "status": "declared",
              "provenance": {
                "page": 16,
                "section": "",
                "table": "",
                "module": "A4",
                "unit_raw": "kg CO2 eq"
              }
            },
            "A5": {
              "value": 12.9,
              "raw": "12.9",
              "status": "declared",
              "provenance": {
                "page": 16,
                "section": "",
                "table": "",
                "module": "A5",
                "unit_raw": "kg CO2 eq"
              }
            },
            "C1": {
              "value": 0.522,
              "raw": "0.522",
              "status": "declared",
              "provenance": {
                "page": 16,
                "section": "",
                "table": "",
                "module": "C1",
                "unit_raw": "kg CO2 eq"
              }
            },
            "C2": {
              "value": 4.31,
              "raw": "4.31",
              "status": "declared",
              "provenance": {
                "page": 16,
                "section": "",
                "table": "",
                "module": "C2",
                "unit_raw": "kg CO2 eq"
              }
            },
            "C3": {
              "value": 10.4,
              "raw": "10.4",
              "status": "declared",
              "provenance": {
                "page": 16,
                "section": "",
                "table": "",
                "module": "C3",
                "unit_raw": "kg CO2 eq"
              }
            },
            "C4": {
              "value": 0.0,
              "raw": "0",
              "status": "declared_zero",
              "provenance": {
                "page": 16,
                "section": "",
                "table": "",
                "module": "C4",
                "unit_raw": "kg CO2 eq"
              }
            },
            "D": {
              "value": -18.5,
              "raw": "-18.5",
              "status": "declared",
              "provenance": {
                "page": 16,
                "section": "",
                "table": "",
                "module": "D",
                "unit_raw": "kg CO2 eq"
              }
            }
          }
        },
        "GWP_fossil": {
          "unit_raw": "kg CO2 eq",
          "unit_normalised": "kg CO2e",
          "header_modules": [
            "A1-A3",
            "A4",
            "A5",
            "C1",
            "C2",
            "C3",
            "C4",
            "D"
          ],
          "modules": {
            "A1-A3": {
              "value": 145.0,
              "raw": "145",
              "status": "declared",
              "provenance": {
                "page": 16,
                "section": "",
                "table": "",
                "module": "A1-A3",
                "unit_raw": "kg CO2 eq"
              }
            },
            "A4": {
              "value": 2.58,
              "raw": "2.58",
              "status": "declared",
              "provenance": {
                "page": 16,
                "section": "",
                "table": "",
                "module": "A4",
                "unit_raw": "kg CO2 eq"
              }
            },
            "A5": {
              "value": 12.8,
              "raw": "12.8",
              "status": "declared",
              "provenance": {
                "page": 16,
                "section": "",
                "table": "",
                "module": "A5",
                "unit_raw": "kg CO2 eq"
              }
            },
            "C1": {
              "value": 0.522,
              "raw": "0.522",
              "status": "declared",
              "provenance": {
                "page": 16,
                "section": "",
                "table": "",
                "module": "C1",
                "unit_raw": "kg CO2 eq"
              }
            },
            "C2": {
              "value": 4.31,
              "raw": "4.31",
              "status": "declared",
              "provenance": {
                "page": 16,
                "section": "",
                "table": "",
                "module": "C2",
                "unit_raw": "kg CO2 eq"
              }
            },
            "C3": {
              "value": 10.3,
              "raw": "10.3",
              "status": "declared",
              "provenance": {
                "page": 16,
                "section": "",
                "table": "",
                "module": "C3",
                "unit_raw": "kg CO2 eq"
              }
            },
            "C4": {
              "value": 0.0,
              "raw": "0",
              "status": "declared_zero",
              "provenance": {
                "page": 16,
                "section": "",
                "table": "",
                "module": "C4",
                "unit_raw": "kg CO2 eq"
              }
            },
            "D": {
              "value": -18.5,
              "raw": "-18.5",
              "status": "declared",
              "provenance": {
                "page": 16,
                "section": "",
                "table": "",
                "module": "D",
                "unit_raw": "kg CO2 eq"
              }
            }
          }
        },
        "GWP_biogenic": {
          "unit_raw": "kg CO2 eq",
          "unit_normalised": "kg CO2e",
          "header_modules": [
            "A1-A3",
            "A4",
            "A5",
            "C1",
            "C2",
            "C3",
            "C4",
            "D"
          ],
          "modules": {
            "A1-A3": {
              "value": 0.822,
              "raw": "0.822",
              "status": "declared",
              "provenance": {
                "page": 16,
                "section": "",
                "table": "",
                "module": "A1-A3",
                "unit_raw": "kg CO2 eq"
              }
            },
            "A4": {
              "value": 8.96e-05,
              "raw": "0.0000896",
              "status": "declared",
              "provenance": {
                "page": 16,
                "section": "",
                "table": "",
                "module": "A4",
                "unit_raw": "kg CO2 eq"
              }
            },
            "A5": {
              "value": 0.0299,
              "raw": "0.0299",
              "status": "declared",
              "provenance": {
                "page": 16,
                "section": "",
                "table": "",
                "module": "A5",
                "unit_raw": "kg CO2 eq"
              }
            },
            "C1": {
              "value": 2.23e-05,
              "raw": "0.0000223",
              "status": "declared",
              "provenance": {
                "page": 16,
                "section": "",
                "table": "",
                "module": "C1",
                "unit_raw": "kg CO2 eq"
              }
            },
            "C2": {
              "value": 0.00015,
              "raw": "0.000150",
              "status": "declared",
              "provenance": {
                "page": 16,
                "section": "",
                "table": "",
                "module": "C2",
                "unit_raw": "kg CO2 eq"
              }
            },
            "C3": {
              "value": 0.00865,
              "raw": "0.00865",
              "status": "declared",
              "provenance": {
                "page": 16,
                "section": "",
                "table": "",
                "module": "C3",
                "unit_raw": "kg CO2 eq"
              }
            },
            "C4": {
              "value": 0.0,
              "raw": "0",
              "status": "declared_zero",
              "provenance": {
                "page": 16,
                "section": "",
                "table": "",
                "module": "C4",
                "unit_raw": "kg CO2 eq"
              }
            },
            "D": {
              "value": -0.015,
              "raw": "-0.0150",
              "status": "declared",
              "provenance": {
                "page": 16,
                "section": "",
                "table": "",
                "module": "D",
                "unit_raw": "kg CO2 eq"
              }
            }
          }
        },
        "GWP_luluc": {
          "unit_raw": "kg CO2 eq",
          "unit_normalised": "kg CO2e",
          "header_modules": [
            "A1-A3",
            "A4",
            "A5",
            "C1",
            "C2",
            "C3",
            "C4",
            "D"
          ],
          "modules": {
            "A1-A3": {
              "value": 0.0489,
              "raw": "0.0489",
              "status": "declared",
              "provenance": {
                "page": 16,
                "section": "",
                "table": "",
                "module": "A1-A3",
                "unit_raw": "kg CO2 eq"
              }
            },
            "A4": {
              "value": 6.61e-05,
              "raw": "0.0000661",
              "status": "declared",
              "provenance": {
                "page": 16,
                "section": "",
                "table": "",
                "module": "A4",
                "unit_raw": "kg CO2 eq"
              }
            },
            "A5": {
              "value": 0.0104,
              "raw": "0.0104",
              "status": "declared",
              "provenance": {
                "page": 16,
                "section": "",
                "table": "",
                "module": "A5",
                "unit_raw": "kg CO2 eq"
              }
            },
            "C1": {
              "value": 1.84e-05,
              "raw": "0.0000184",
              "status": "declared",
              "provenance": {
                "page": 16,
                "section": "",
                "table": "",
                "module": "C1",
                "unit_raw": "kg CO2 eq"
              }
            },
            "C2": {
              "value": 0.00011,
              "raw": "0.000110",
              "status": "declared",
              "provenance": {
                "page": 16,
                "section": "",
                "table": "",
                "module": "C2",
                "unit_raw": "kg CO2 eq"
              }
            },
            "C3": {
              "value": 0.0081,
              "raw": "0.00810",
              "status": "declared",
              "provenance": {
                "page": 16,
                "section": "",
                "table": "",
                "module": "C3",
                "unit_raw": "kg CO2 eq"
              }
            },
            "C4": {
              "value": 0.0,
              "raw": "0",
              "status": "declared_zero",
              "provenance": {
                "page": 16,
                "section": "",
                "table": "",
                "module": "C4",
                "unit_raw": "kg CO2 eq"
              }
            },
            "D": {
              "value": -0.0168,
              "raw": "-0.0168",
              "status": "declared",
              "provenance": {
                "page": 16,
                "section": "",
                "table": "",
                "module": "D",
                "unit_raw": "kg CO2 eq"
              }
            }
          }
        },
        "GWP_GHG": {
          "unit_raw": "kg CO2 eq",
          "unit_normalised": "kg CO2e",
          "header_modules": [
            "A1-A3",
            "A4",
            "A5",
            "C1",
            "C2",
            "C3",
            "C4",
            "D"
          ],
          "modules": {
            "A1-A3": {
              "value": 146.0,
              "raw": "146",
              "status": "declared",
              "provenance": {
                "page": 17,
                "section": "",
                "table": "",
                "module": "A1-A3",
                "unit_raw": "kg CO2 eq"
              }
            },
            "A4": {
              "value": 2.58,
              "raw": "2.58",
              "status": "declared",
              "provenance": {
                "page": 17,
                "section": "",
                "table": "",
                "module": "A4",
                "unit_raw": "kg CO2 eq"
              }
            },
            "A5": {
              "value": 12.9,
              "raw": "12.9",
              "status": "declared",
              "provenance": {
                "page": 17,
                "section": "",
                "table": "",
                "module": "A5",
                "unit_raw": "kg CO2 eq"
              }
            },
            "C1": {
              "value": 0.522,
              "raw": "0.522",
              "status": "declared",
              "provenance": {
                "page": 17,
                "section": "",
                "table": "",
                "module": "C1",
                "unit_raw": "kg CO2 eq"
              }
            },
            "C2": {
              "value": 4.31,
              "raw": "4.31",
              "status": "declared",
              "provenance": {
                "page": 17,
                "section": "",
                "table": "",
                "module": "C2",
                "unit_raw": "kg CO2 eq"
              }
            },
            "C3": {
              "value": 10.4,
              "raw": "10.4",
              "status": "declared",
              "provenance": {
                "page": 17,
                "section": "",
                "table": "",
                "module": "C3",
                "unit_raw": "kg CO2 eq"
              }
            },
            "C4": {
              "value": 0.0,
              "raw": "0",
              "status": "declared_zero",
              "provenance": {
                "page": 17,
                "section": "",
                "table": "",
                "module": "C4",
                "unit_raw": "kg CO2 eq"
              }
            },
            "D": {
              "value": -18.5,
              "raw": "-18.5",
              "status": "declared",
              "provenance": {
                "page": 17,
                "section": "",
                "table": "",
                "module": "D",
                "unit_raw": "kg CO2 eq"
              }
            }
          }
        }
      }
    }
  ],
  "system_boundary": {
    "A1": "declared",
    "A2": "declared",
    "A3": "declared",
    "A1-A3": "declared",
    "A4": "declared",
    "A5": "declared",
    "B1": "not_declared",
    "B2": "not_declared",
    "B3": "not_declared",
    "B4": "not_declared",
    "B5": "not_declared",
    "B6": "not_declared",
    "B7": "not_declared",
    "C1": "declared",
    "C2": "declared",
    "C3": "declared",
    "C4": "declared",
    "D": "declared"
  },
  "comparability_notes": [
    "Cradle-to-gate (A1-A3) with options A4-A5, full C1-C4 and module D declared; use stage B1-B7 not declared (ND).",
    "C4 GWP prints 0 on page 16 (declared value, status declared not not_declared).",
    "Lower-carbon ECOPact range; multi-plant Brisbane EPD under Holcim's certified EPD Process (process certification, no pre-verified LCA/EPD tool).",
    "GWP-GHG table shows minor rounding differences vs GWP-Total: A1-A3 146 vs 148, A4 2.58 vs 2.59, C1 0.522 vs 0.523, C2 4.31 vs 4.32 — flagged, numbers not changed.",
    "Declared unit 1 m3; product mass 2319 kg/m3."
  ],
  "extraction_meta": {
    "method": "deterministic coordinate/order-bound table parse; contextual fields agent-verified",
    "numbers_validated": "cross_validate.py (raw string present on cited page)",
    "verified_by": "epd-context-agent (opus)",
    "checked_by": null,
    "confidence": "high",
    "warnings": [
      "Cell conflict across pages: GWP_GHG.A1-A3: '146' vs '148'",
      "Cell conflict across pages: GWP_GHG.A4: '2.58' vs '2.59'",
      "Cell conflict across pages: GWP_GHG.C1: '0.522' vs '0.523'",
      "Cell conflict across pages: GWP_GHG.C2: '4.31' vs '4.32'",
      "GWP-GHG vs GWP-Total rounding conflicts present in candidate extraction_meta (A1-A3 146/148, A4 2.58/2.59, C1 0.522/0.523, C2 4.31/4.32). GWP-Total values on page 16 confirmed correct."
    ],
    "needs_review": []
  }
}