{
  "schema_version": "1.0",
  "epd": {
    "id": "EPD_HUB-5991",
    "source_pdf": "EPD_HUB-5991_2026-06-27_en.pdf",
    "pages": 13,
    "program_operator": "EPD Hub, hub@epdhub.com",
    "pcr": "EPD Hub Core PCR version 1.2, 24 Mar 2025",
    "reference_standard": "EN 15804:2012+A2:2019/AC:2021",
    "en15804_version": "A2",
    "characterisation": "EF 3.1",
    "published": "15.04.2026",
    "valid_until": "14.04.2031",
    "provenance": {
      "program_operator": {
        "page": 2,
        "snippet": "Program operator | EPD Hub, hub@epdhub.com"
      },
      "pcr": {
        "page": 2,
        "snippet": "PCR | EPD Hub Core PCR version 1.2, 24 Mar 2025"
      },
      "published": {
        "page": 1,
        "snippet": "Published on 15.04.2026"
      },
      "valid_until": {
        "page": 1,
        "snippet": "valid until 14.04.2031"
      }
    },
    "page_labels": null
  },
  "products": [
    {
      "name": "N40/20 Xencrete",
      "manufacturer": "Entire Concrete",
      "concrete_type": "Ready-mix concrete",
      "compressive_strength": {
        "value_mpa": 40,
        "class": "N40",
        "at_days": null,
        "raw": null,
        "status": "found",
        "provenance": {
          "page": 2,
          "snippet": "characteristic strength of 40MPa"
        }
      },
      "manufacturing_location": {
        "site": "Hunter Valley, NSW",
        "city": "Hunter Valley",
        "region": "New South Wales",
        "country": "AU",
        "raw": "Hunter Valley, NSW",
        "provenance": {
          "page": 2,
          "snippet": "Manufacturer Entire Concrete; Place of production Hunter Valley, NSW"
        }
      },
      "declared_unit": {
        "amount": 1,
        "unit": "m3",
        "description": "1 cubic meter",
        "mass_kg": 2306.0,
        "provenance": {
          "page": 2,
          "snippet": "Declared unit | 1 cubic meter"
        }
      },
      "indicators": {
        "GWP_total": {
          "unit_raw": "kg CO2e",
          "unit_normalised": "kg CO2e",
          "header_modules": [
            "A1",
            "A2",
            "A3",
            "A1-A3",
            "A4",
            "A5",
            "B1",
            "B2",
            "B3",
            "B4",
            "B5",
            "B6",
            "B7",
            "C1",
            "C2",
            "C3",
            "C4",
            "D"
          ],
          "modules": {
            "A1": {
              "value": 235.0,
              "raw": "2.35E+02",
              "status": "declared",
              "provenance": {
                "page": 8,
                "section": "CORE ENVIRONMENTAL IMPACT INDICATORS – EN 15804+A2, EF 3.1",
                "table": "CORE ENVIRONMENTAL IMPACT INDICATORS – EN 15804+A2, EF 3.1",
                "module": "A1",
                "unit_raw": "kg CO2e"
              }
            },
            "A2": {
              "value": 34.2,
              "raw": "3.42E+01",
              "status": "declared",
              "provenance": {
                "page": 8,
                "section": "CORE ENVIRONMENTAL IMPACT INDICATORS – EN 15804+A2, EF 3.1",
                "table": "CORE ENVIRONMENTAL IMPACT INDICATORS – EN 15804+A2, EF 3.1",
                "module": "A2",
                "unit_raw": "kg CO2e"
              }
            },
            "A3": {
              "value": 3.71,
              "raw": "3.71E+00",
              "status": "declared",
              "provenance": {
                "page": 8,
                "section": "CORE ENVIRONMENTAL IMPACT INDICATORS – EN 15804+A2, EF 3.1",
                "table": "CORE ENVIRONMENTAL IMPACT INDICATORS – EN 15804+A2, EF 3.1",
                "module": "A3",
                "unit_raw": "kg CO2e"
              }
            },
            "A1-A3": {
              "value": 273.0,
              "raw": "2.73E+02",
              "status": "declared",
              "provenance": {
                "page": 8,
                "section": "CORE ENVIRONMENTAL IMPACT INDICATORS – EN 15804+A2, EF 3.1",
                "table": "CORE ENVIRONMENTAL IMPACT INDICATORS – EN 15804+A2, EF 3.1",
                "module": "A1-A3",
                "unit_raw": "kg CO2e"
              }
            },
            "A4": {
              "value": 2.96,
              "raw": "2.96E+00",
              "status": "declared",
              "provenance": {
                "page": 8,
                "section": "CORE ENVIRONMENTAL IMPACT INDICATORS – EN 15804+A2, EF 3.1",
                "table": "CORE ENVIRONMENTAL IMPACT INDICATORS – EN 15804+A2, EF 3.1",
                "module": "A4",
                "unit_raw": "kg CO2e"
              }
            },
            "A5": {
              "value": 16.4,
              "raw": "1.64E+01",
              "status": "declared",
              "provenance": {
                "page": 8,
                "section": "CORE ENVIRONMENTAL IMPACT INDICATORS – EN 15804+A2, EF 3.1",
                "table": "CORE ENVIRONMENTAL IMPACT INDICATORS – EN 15804+A2, EF 3.1",
                "module": "A5",
                "unit_raw": "kg CO2e"
              }
            },
            "B1": {
              "value": null,
              "raw": "ND",
              "status": "not_declared",
              "provenance": {
                "page": 8,
                "section": "CORE ENVIRONMENTAL IMPACT INDICATORS – EN 15804+A2, EF 3.1",
                "table": "CORE ENVIRONMENTAL IMPACT INDICATORS – EN 15804+A2, EF 3.1",
                "module": "B1",
                "unit_raw": "kg CO2e"
              }
            },
            "B2": {
              "value": null,
              "raw": "ND",
              "status": "not_declared",
              "provenance": {
                "page": 8,
                "section": "CORE ENVIRONMENTAL IMPACT INDICATORS – EN 15804+A2, EF 3.1",
                "table": "CORE ENVIRONMENTAL IMPACT INDICATORS – EN 15804+A2, EF 3.1",
                "module": "B2",
                "unit_raw": "kg CO2e"
              }
            },
            "B3": {
              "value": null,
              "raw": "ND",
              "status": "not_declared",
              "provenance": {
                "page": 8,
                "section": "CORE ENVIRONMENTAL IMPACT INDICATORS – EN 15804+A2, EF 3.1",
                "table": "CORE ENVIRONMENTAL IMPACT INDICATORS – EN 15804+A2, EF 3.1",
                "module": "B3",
                "unit_raw": "kg CO2e"
              }
            },
            "B4": {
              "value": null,
              "raw": "ND",
              "status": "not_declared",
              "provenance": {
                "page": 8,
                "section": "CORE ENVIRONMENTAL IMPACT INDICATORS – EN 15804+A2, EF 3.1",
                "table": "CORE ENVIRONMENTAL IMPACT INDICATORS – EN 15804+A2, EF 3.1",
                "module": "B4",
                "unit_raw": "kg CO2e"
              }
            },
            "B5": {
              "value": null,
              "raw": "ND",
              "status": "not_declared",
              "provenance": {
                "page": 8,
                "section": "CORE ENVIRONMENTAL IMPACT INDICATORS – EN 15804+A2, EF 3.1",
                "table": "CORE ENVIRONMENTAL IMPACT INDICATORS – EN 15804+A2, EF 3.1",
                "module": "B5",
                "unit_raw": "kg CO2e"
              }
            },
            "B6": {
              "value": null,
              "raw": "ND",
              "status": "not_declared",
              "provenance": {
                "page": 8,
                "section": "CORE ENVIRONMENTAL IMPACT INDICATORS – EN 15804+A2, EF 3.1",
                "table": "CORE ENVIRONMENTAL IMPACT INDICATORS – EN 15804+A2, EF 3.1",
                "module": "B6",
                "unit_raw": "kg CO2e"
              }
            },
            "B7": {
              "value": null,
              "raw": "ND",
              "status": "not_declared",
              "provenance": {
                "page": 8,
                "section": "CORE ENVIRONMENTAL IMPACT INDICATORS – EN 15804+A2, EF 3.1",
                "table": "CORE ENVIRONMENTAL IMPACT INDICATORS – EN 15804+A2, EF 3.1",
                "module": "B7",
                "unit_raw": "kg CO2e"
              }
            },
            "C1": {
              "value": 4.39,
              "raw": "4.39E+00",
              "status": "declared",
              "provenance": {
                "page": 8,
                "section": "CORE ENVIRONMENTAL IMPACT INDICATORS – EN 15804+A2, EF 3.1",
                "table": "CORE ENVIRONMENTAL IMPACT INDICATORS – EN 15804+A2, EF 3.1",
                "module": "C1",
                "unit_raw": "kg CO2e"
              }
            },
            "C2": {
              "value": 12.4,
              "raw": "1.24E+01",
              "status": "declared",
              "provenance": {
                "page": 8,
                "section": "CORE ENVIRONMENTAL IMPACT INDICATORS – EN 15804+A2, EF 3.1",
                "table": "CORE ENVIRONMENTAL IMPACT INDICATORS – EN 15804+A2, EF 3.1",
                "module": "C2",
                "unit_raw": "kg CO2e"
              }
            },
            "C3": {
              "value": 7.06,
              "raw": "7.06E+00",
              "status": "declared",
              "provenance": {
                "page": 8,
                "section": "CORE ENVIRONMENTAL IMPACT INDICATORS – EN 15804+A2, EF 3.1",
                "table": "CORE ENVIRONMENTAL IMPACT INDICATORS – EN 15804+A2, EF 3.1",
                "module": "C3",
                "unit_raw": "kg CO2e"
              }
            },
            "C4": {
              "value": 4.32,
              "raw": "4.32E+00",
              "status": "declared",
              "provenance": {
                "page": 8,
                "section": "CORE ENVIRONMENTAL IMPACT INDICATORS – EN 15804+A2, EF 3.1",
                "table": "CORE ENVIRONMENTAL IMPACT INDICATORS – EN 15804+A2, EF 3.1",
                "module": "C4",
                "unit_raw": "kg CO2e"
              }
            },
            "D": {
              "value": -11.9,
              "raw": "‐1.19E+01",
              "status": "declared",
              "provenance": {
                "page": 8,
                "section": "CORE ENVIRONMENTAL IMPACT INDICATORS – EN 15804+A2, EF 3.1",
                "table": "CORE ENVIRONMENTAL IMPACT INDICATORS – EN 15804+A2, EF 3.1",
                "module": "D",
                "unit_raw": "kg CO2e"
              }
            }
          }
        },
        "GWP_fossil": {
          "unit_raw": "kg CO2e",
          "unit_normalised": "kg CO2e",
          "header_modules": [
            "A1",
            "A2",
            "A3",
            "A1-A3",
            "A4",
            "A5",
            "B1",
            "B2",
            "B3",
            "B4",
            "B5",
            "B6",
            "B7",
            "C1",
            "C2",
            "C3",
            "C4",
            "D"
          ],
          "modules": {
            "A1": {
              "value": 235.0,
              "raw": "2.35E+02",
              "status": "declared",
              "provenance": {
                "page": 8,
                "section": "CORE ENVIRONMENTAL IMPACT INDICATORS – EN 15804+A2, EF 3.1",
                "table": "CORE ENVIRONMENTAL IMPACT INDICATORS – EN 15804+A2, EF 3.1",
                "module": "A1",
                "unit_raw": "kg CO2e"
              }
            },
            "A2": {
              "value": 34.2,
              "raw": "3.42E+01",
              "status": "declared",
              "provenance": {
                "page": 8,
                "section": "CORE ENVIRONMENTAL IMPACT INDICATORS – EN 15804+A2, EF 3.1",
                "table": "CORE ENVIRONMENTAL IMPACT INDICATORS – EN 15804+A2, EF 3.1",
                "module": "A2",
                "unit_raw": "kg CO2e"
              }
            },
            "A3": {
              "value": 3.71,
              "raw": "3.71E+00",
              "status": "declared",
              "provenance": {
                "page": 8,
                "section": "CORE ENVIRONMENTAL IMPACT INDICATORS – EN 15804+A2, EF 3.1",
                "table": "CORE ENVIRONMENTAL IMPACT INDICATORS – EN 15804+A2, EF 3.1",
                "module": "A3",
                "unit_raw": "kg CO2e"
              }
            },
            "A1-A3": {
              "value": 273.0,
              "raw": "2.73E+02",
              "status": "declared",
              "provenance": {
                "page": 8,
                "section": "CORE ENVIRONMENTAL IMPACT INDICATORS – EN 15804+A2, EF 3.1",
                "table": "CORE ENVIRONMENTAL IMPACT INDICATORS – EN 15804+A2, EF 3.1",
                "module": "A1-A3",
                "unit_raw": "kg CO2e"
              }
            },
            "A4": {
              "value": 2.95,
              "raw": "2.95E+00",
              "status": "declared",
              "provenance": {
                "page": 8,
                "section": "CORE ENVIRONMENTAL IMPACT INDICATORS – EN 15804+A2, EF 3.1",
                "table": "CORE ENVIRONMENTAL IMPACT INDICATORS – EN 15804+A2, EF 3.1",
                "module": "A4",
                "unit_raw": "kg CO2e"
              }
            },
            "A5": {
              "value": 16.4,
              "raw": "1.64E+01",
              "status": "declared",
              "provenance": {
                "page": 8,
                "section": "CORE ENVIRONMENTAL IMPACT INDICATORS – EN 15804+A2, EF 3.1",
                "table": "CORE ENVIRONMENTAL IMPACT INDICATORS – EN 15804+A2, EF 3.1",
                "module": "A5",
                "unit_raw": "kg CO2e"
              }
            },
            "B1": {
              "value": null,
              "raw": "ND",
              "status": "not_declared",
              "provenance": {
                "page": 8,
                "section": "CORE ENVIRONMENTAL IMPACT INDICATORS – EN 15804+A2, EF 3.1",
                "table": "CORE ENVIRONMENTAL IMPACT INDICATORS – EN 15804+A2, EF 3.1",
                "module": "B1",
                "unit_raw": "kg CO2e"
              }
            },
            "B2": {
              "value": null,
              "raw": "ND",
              "status": "not_declared",
              "provenance": {
                "page": 8,
                "section": "CORE ENVIRONMENTAL IMPACT INDICATORS – EN 15804+A2, EF 3.1",
                "table": "CORE ENVIRONMENTAL IMPACT INDICATORS – EN 15804+A2, EF 3.1",
                "module": "B2",
                "unit_raw": "kg CO2e"
              }
            },
            "B3": {
              "value": null,
              "raw": "ND",
              "status": "not_declared",
              "provenance": {
                "page": 8,
                "section": "CORE ENVIRONMENTAL IMPACT INDICATORS – EN 15804+A2, EF 3.1",
                "table": "CORE ENVIRONMENTAL IMPACT INDICATORS – EN 15804+A2, EF 3.1",
                "module": "B3",
                "unit_raw": "kg CO2e"
              }
            },
            "B4": {
              "value": null,
              "raw": "ND",
              "status": "not_declared",
              "provenance": {
                "page": 8,
                "section": "CORE ENVIRONMENTAL IMPACT INDICATORS – EN 15804+A2, EF 3.1",
                "table": "CORE ENVIRONMENTAL IMPACT INDICATORS – EN 15804+A2, EF 3.1",
                "module": "B4",
                "unit_raw": "kg CO2e"
              }
            },
            "B5": {
              "value": null,
              "raw": "ND",
              "status": "not_declared",
              "provenance": {
                "page": 8,
                "section": "CORE ENVIRONMENTAL IMPACT INDICATORS – EN 15804+A2, EF 3.1",
                "table": "CORE ENVIRONMENTAL IMPACT INDICATORS – EN 15804+A2, EF 3.1",
                "module": "B5",
                "unit_raw": "kg CO2e"
              }
            },
            "B6": {
              "value": null,
              "raw": "ND",
              "status": "not_declared",
              "provenance": {
                "page": 8,
                "section": "CORE ENVIRONMENTAL IMPACT INDICATORS – EN 15804+A2, EF 3.1",
                "table": "CORE ENVIRONMENTAL IMPACT INDICATORS – EN 15804+A2, EF 3.1",
                "module": "B6",
                "unit_raw": "kg CO2e"
              }
            },
            "B7": {
              "value": null,
              "raw": "ND",
              "status": "not_declared",
              "provenance": {
                "page": 8,
                "section": "CORE ENVIRONMENTAL IMPACT INDICATORS – EN 15804+A2, EF 3.1",
                "table": "CORE ENVIRONMENTAL IMPACT INDICATORS – EN 15804+A2, EF 3.1",
                "module": "B7",
                "unit_raw": "kg CO2e"
              }
            },
            "C1": {
              "value": 4.39,
              "raw": "4.39E+00",
              "status": "declared",
              "provenance": {
                "page": 8,
                "section": "CORE ENVIRONMENTAL IMPACT INDICATORS – EN 15804+A2, EF 3.1",
                "table": "CORE ENVIRONMENTAL IMPACT INDICATORS – EN 15804+A2, EF 3.1",
                "module": "C1",
                "unit_raw": "kg CO2e"
              }
            },
            "C2": {
              "value": 12.4,
              "raw": "1.24E+01",
              "status": "declared",
              "provenance": {
                "page": 8,
                "section": "CORE ENVIRONMENTAL IMPACT INDICATORS – EN 15804+A2, EF 3.1",
                "table": "CORE ENVIRONMENTAL IMPACT INDICATORS – EN 15804+A2, EF 3.1",
                "module": "C2",
                "unit_raw": "kg CO2e"
              }
            },
            "C3": {
              "value": 7.06,
              "raw": "7.06E+00",
              "status": "declared",
              "provenance": {
                "page": 8,
                "section": "CORE ENVIRONMENTAL IMPACT INDICATORS – EN 15804+A2, EF 3.1",
                "table": "CORE ENVIRONMENTAL IMPACT INDICATORS – EN 15804+A2, EF 3.1",
                "module": "C3",
                "unit_raw": "kg CO2e"
              }
            },
            "C4": {
              "value": 4.32,
              "raw": "4.32E+00",
              "status": "declared",
              "provenance": {
                "page": 8,
                "section": "CORE ENVIRONMENTAL IMPACT INDICATORS – EN 15804+A2, EF 3.1",
                "table": "CORE ENVIRONMENTAL IMPACT INDICATORS – EN 15804+A2, EF 3.1",
                "module": "C4",
                "unit_raw": "kg CO2e"
              }
            },
            "D": {
              "value": -11.8,
              "raw": "‐1.18E+01",
              "status": "declared",
              "provenance": {
                "page": 8,
                "section": "CORE ENVIRONMENTAL IMPACT INDICATORS – EN 15804+A2, EF 3.1",
                "table": "CORE ENVIRONMENTAL IMPACT INDICATORS – EN 15804+A2, EF 3.1",
                "module": "D",
                "unit_raw": "kg CO2e"
              }
            }
          }
        },
        "GWP_biogenic": {
          "unit_raw": "kg CO2e",
          "unit_normalised": "kg CO2e",
          "header_modules": [
            "A1",
            "A2",
            "A3",
            "A1-A3",
            "A4",
            "A5",
            "B1",
            "B2",
            "B3",
            "B4",
            "B5",
            "B6",
            "B7",
            "C1",
            "C2",
            "C3",
            "C4",
            "D"
          ],
          "modules": {
            "A1": {
              "value": 0.095,
              "raw": "9.50E‐02",
              "status": "declared",
              "provenance": {
                "page": 8,
                "section": "CORE ENVIRONMENTAL IMPACT INDICATORS – EN 15804+A2, EF 3.1",
                "table": "CORE ENVIRONMENTAL IMPACT INDICATORS – EN 15804+A2, EF 3.1",
                "module": "A1",
                "unit_raw": "kg CO2e"
              }
            },
            "A2": {
              "value": 0.00711,
              "raw": "7.11E‐03",
              "status": "declared",
              "provenance": {
                "page": 8,
                "section": "CORE ENVIRONMENTAL IMPACT INDICATORS – EN 15804+A2, EF 3.1",
                "table": "CORE ENVIRONMENTAL IMPACT INDICATORS – EN 15804+A2, EF 3.1",
                "module": "A2",
                "unit_raw": "kg CO2e"
              }
            },
            "A3": {
              "value": 0.000621,
              "raw": "6.21E‐04",
              "status": "declared",
              "provenance": {
                "page": 8,
                "section": "CORE ENVIRONMENTAL IMPACT INDICATORS – EN 15804+A2, EF 3.1",
                "table": "CORE ENVIRONMENTAL IMPACT INDICATORS – EN 15804+A2, EF 3.1",
                "module": "A3",
                "unit_raw": "kg CO2e"
              }
            },
            "A1-A3": {
              "value": 0.103,
              "raw": "1.03E‐01",
              "status": "declared",
              "provenance": {
                "page": 8,
                "section": "CORE ENVIRONMENTAL IMPACT INDICATORS – EN 15804+A2, EF 3.1",
                "table": "CORE ENVIRONMENTAL IMPACT INDICATORS – EN 15804+A2, EF 3.1",
                "module": "A1-A3",
                "unit_raw": "kg CO2e"
              }
            },
            "A4": {
              "value": 0.000669,
              "raw": "6.69E‐04",
              "status": "declared",
              "provenance": {
                "page": 8,
                "section": "CORE ENVIRONMENTAL IMPACT INDICATORS – EN 15804+A2, EF 3.1",
                "table": "CORE ENVIRONMENTAL IMPACT INDICATORS – EN 15804+A2, EF 3.1",
                "module": "A4",
                "unit_raw": "kg CO2e"
              }
            },
            "A5": {
              "value": 0.00388,
              "raw": "3.88E‐03",
              "status": "declared",
              "provenance": {
                "page": 8,
                "section": "CORE ENVIRONMENTAL IMPACT INDICATORS – EN 15804+A2, EF 3.1",
                "table": "CORE ENVIRONMENTAL IMPACT INDICATORS – EN 15804+A2, EF 3.1",
                "module": "A5",
                "unit_raw": "kg CO2e"
              }
            },
            "B1": {
              "value": null,
              "raw": "ND",
              "status": "not_declared",
              "provenance": {
                "page": 8,
                "section": "CORE ENVIRONMENTAL IMPACT INDICATORS – EN 15804+A2, EF 3.1",
                "table": "CORE ENVIRONMENTAL IMPACT INDICATORS – EN 15804+A2, EF 3.1",
                "module": "B1",
                "unit_raw": "kg CO2e"
              }
            },
            "B2": {
              "value": null,
              "raw": "ND",
              "status": "not_declared",
              "provenance": {
                "page": 8,
                "section": "CORE ENVIRONMENTAL IMPACT INDICATORS – EN 15804+A2, EF 3.1",
                "table": "CORE ENVIRONMENTAL IMPACT INDICATORS – EN 15804+A2, EF 3.1",
                "module": "B2",
                "unit_raw": "kg CO2e"
              }
            },
            "B3": {
              "value": null,
              "raw": "ND",
              "status": "not_declared",
              "provenance": {
                "page": 8,
                "section": "CORE ENVIRONMENTAL IMPACT INDICATORS – EN 15804+A2, EF 3.1",
                "table": "CORE ENVIRONMENTAL IMPACT INDICATORS – EN 15804+A2, EF 3.1",
                "module": "B3",
                "unit_raw": "kg CO2e"
              }
            },
            "B4": {
              "value": null,
              "raw": "ND",
              "status": "not_declared",
              "provenance": {
                "page": 8,
                "section": "CORE ENVIRONMENTAL IMPACT INDICATORS – EN 15804+A2, EF 3.1",
                "table": "CORE ENVIRONMENTAL IMPACT INDICATORS – EN 15804+A2, EF 3.1",
                "module": "B4",
                "unit_raw": "kg CO2e"
              }
            },
            "B5": {
              "value": null,
              "raw": "ND",
              "status": "not_declared",
              "provenance": {
                "page": 8,
                "section": "CORE ENVIRONMENTAL IMPACT INDICATORS – EN 15804+A2, EF 3.1",
                "table": "CORE ENVIRONMENTAL IMPACT INDICATORS – EN 15804+A2, EF 3.1",
                "module": "B5",
                "unit_raw": "kg CO2e"
              }
            },
            "B6": {
              "value": null,
              "raw": "ND",
              "status": "not_declared",
              "provenance": {
                "page": 8,
                "section": "CORE ENVIRONMENTAL IMPACT INDICATORS – EN 15804+A2, EF 3.1",
                "table": "CORE ENVIRONMENTAL IMPACT INDICATORS – EN 15804+A2, EF 3.1",
                "module": "B6",
                "unit_raw": "kg CO2e"
              }
            },
            "B7": {
              "value": null,
              "raw": "ND",
              "status": "not_declared",
              "provenance": {
                "page": 8,
                "section": "CORE ENVIRONMENTAL IMPACT INDICATORS – EN 15804+A2, EF 3.1",
                "table": "CORE ENVIRONMENTAL IMPACT INDICATORS – EN 15804+A2, EF 3.1",
                "module": "B7",
                "unit_raw": "kg CO2e"
              }
            },
            "C1": {
              "value": 0.000448,
              "raw": "4.48E‐04",
              "status": "declared",
              "provenance": {
                "page": 8,
                "section": "CORE ENVIRONMENTAL IMPACT INDICATORS – EN 15804+A2, EF 3.1",
                "table": "CORE ENVIRONMENTAL IMPACT INDICATORS – EN 15804+A2, EF 3.1",
                "module": "C1",
                "unit_raw": "kg CO2e"
              }
            },
            "C2": {
              "value": 0.00281,
              "raw": "2.81E‐03",
              "status": "declared",
              "provenance": {
                "page": 8,
                "section": "CORE ENVIRONMENTAL IMPACT INDICATORS – EN 15804+A2, EF 3.1",
                "table": "CORE ENVIRONMENTAL IMPACT INDICATORS – EN 15804+A2, EF 3.1",
                "module": "C2",
                "unit_raw": "kg CO2e"
              }
            },
            "C3": {
              "value": -0.000721,
              "raw": "‐7.21E‐04",
              "status": "declared",
              "provenance": {
                "page": 8,
                "section": "CORE ENVIRONMENTAL IMPACT INDICATORS – EN 15804+A2, EF 3.1",
                "table": "CORE ENVIRONMENTAL IMPACT INDICATORS – EN 15804+A2, EF 3.1",
                "module": "C3",
                "unit_raw": "kg CO2e"
              }
            },
            "C4": {
              "value": -0.00137,
              "raw": "‐1.37E‐03",
              "status": "declared",
              "provenance": {
                "page": 8,
                "section": "CORE ENVIRONMENTAL IMPACT INDICATORS – EN 15804+A2, EF 3.1",
                "table": "CORE ENVIRONMENTAL IMPACT INDICATORS – EN 15804+A2, EF 3.1",
                "module": "C4",
                "unit_raw": "kg CO2e"
              }
            },
            "D": {
              "value": -0.0371,
              "raw": "‐3.71E‐02",
              "status": "declared",
              "provenance": {
                "page": 8,
                "section": "CORE ENVIRONMENTAL IMPACT INDICATORS – EN 15804+A2, EF 3.1",
                "table": "CORE ENVIRONMENTAL IMPACT INDICATORS – EN 15804+A2, EF 3.1",
                "module": "D",
                "unit_raw": "kg CO2e"
              }
            }
          }
        },
        "GWP_luluc": {
          "unit_raw": "kg CO2e",
          "unit_normalised": "kg CO2e",
          "header_modules": [
            "A1",
            "A2",
            "A3",
            "A1-A3",
            "A4",
            "A5",
            "B1",
            "B2",
            "B3",
            "B4",
            "B5",
            "B6",
            "B7",
            "C1",
            "C2",
            "C3",
            "C4",
            "D"
          ],
          "modules": {
            "A1": {
              "value": 0.0378,
              "raw": "3.78E‐02",
              "status": "declared",
              "provenance": {
                "page": 8,
                "section": "CORE ENVIRONMENTAL IMPACT INDICATORS – EN 15804+A2, EF 3.1",
                "table": "CORE ENVIRONMENTAL IMPACT INDICATORS – EN 15804+A2, EF 3.1",
                "module": "A1",
                "unit_raw": "kg CO2e"
              }
            },
            "A2": {
              "value": 0.0184,
              "raw": "1.84E‐02",
              "status": "declared",
              "provenance": {
                "page": 8,
                "section": "CORE ENVIRONMENTAL IMPACT INDICATORS – EN 15804+A2, EF 3.1",
                "table": "CORE ENVIRONMENTAL IMPACT INDICATORS – EN 15804+A2, EF 3.1",
                "module": "A2",
                "unit_raw": "kg CO2e"
              }
            },
            "A3": {
              "value": 0.0003,
              "raw": "3.00E‐04",
              "status": "declared",
              "provenance": {
                "page": 8,
                "section": "CORE ENVIRONMENTAL IMPACT INDICATORS – EN 15804+A2, EF 3.1",
                "table": "CORE ENVIRONMENTAL IMPACT INDICATORS – EN 15804+A2, EF 3.1",
                "module": "A3",
                "unit_raw": "kg CO2e"
              }
            },
            "A1-A3": {
              "value": 0.0565,
              "raw": "5.65E‐02",
              "status": "declared",
              "provenance": {
                "page": 8,
                "section": "CORE ENVIRONMENTAL IMPACT INDICATORS – EN 15804+A2, EF 3.1",
                "table": "CORE ENVIRONMENTAL IMPACT INDICATORS – EN 15804+A2, EF 3.1",
                "module": "A1-A3",
                "unit_raw": "kg CO2e"
              }
            },
            "A4": {
              "value": 0.00132,
              "raw": "1.32E‐03",
              "status": "declared",
              "provenance": {
                "page": 8,
                "section": "CORE ENVIRONMENTAL IMPACT INDICATORS – EN 15804+A2, EF 3.1",
                "table": "CORE ENVIRONMENTAL IMPACT INDICATORS – EN 15804+A2, EF 3.1",
                "module": "A4",
                "unit_raw": "kg CO2e"
              }
            },
            "A5": {
              "value": 0.00275,
              "raw": "2.75E‐03",
              "status": "declared",
              "provenance": {
                "page": 8,
                "section": "CORE ENVIRONMENTAL IMPACT INDICATORS – EN 15804+A2, EF 3.1",
                "table": "CORE ENVIRONMENTAL IMPACT INDICATORS – EN 15804+A2, EF 3.1",
                "module": "A5",
                "unit_raw": "kg CO2e"
              }
            },
            "B1": {
              "value": null,
              "raw": "ND",
              "status": "not_declared",
              "provenance": {
                "page": 8,
                "section": "CORE ENVIRONMENTAL IMPACT INDICATORS – EN 15804+A2, EF 3.1",
                "table": "CORE ENVIRONMENTAL IMPACT INDICATORS – EN 15804+A2, EF 3.1",
                "module": "B1",
                "unit_raw": "kg CO2e"
              }
            },
            "B2": {
              "value": null,
              "raw": "ND",
              "status": "not_declared",
              "provenance": {
                "page": 8,
                "section": "CORE ENVIRONMENTAL IMPACT INDICATORS – EN 15804+A2, EF 3.1",
                "table": "CORE ENVIRONMENTAL IMPACT INDICATORS – EN 15804+A2, EF 3.1",
                "module": "B2",
                "unit_raw": "kg CO2e"
              }
            },
            "B3": {
              "value": null,
              "raw": "ND",
              "status": "not_declared",
              "provenance": {
                "page": 8,
                "section": "CORE ENVIRONMENTAL IMPACT INDICATORS – EN 15804+A2, EF 3.1",
                "table": "CORE ENVIRONMENTAL IMPACT INDICATORS – EN 15804+A2, EF 3.1",
                "module": "B3",
                "unit_raw": "kg CO2e"
              }
            },
            "B4": {
              "value": null,
              "raw": "ND",
              "status": "not_declared",
              "provenance": {
                "page": 8,
                "section": "CORE ENVIRONMENTAL IMPACT INDICATORS – EN 15804+A2, EF 3.1",
                "table": "CORE ENVIRONMENTAL IMPACT INDICATORS – EN 15804+A2, EF 3.1",
                "module": "B4",
                "unit_raw": "kg CO2e"
              }
            },
            "B5": {
              "value": null,
              "raw": "ND",
              "status": "not_declared",
              "provenance": {
                "page": 8,
                "section": "CORE ENVIRONMENTAL IMPACT INDICATORS – EN 15804+A2, EF 3.1",
                "table": "CORE ENVIRONMENTAL IMPACT INDICATORS – EN 15804+A2, EF 3.1",
                "module": "B5",
                "unit_raw": "kg CO2e"
              }
            },
            "B6": {
              "value": null,
              "raw": "ND",
              "status": "not_declared",
              "provenance": {
                "page": 8,
                "section": "CORE ENVIRONMENTAL IMPACT INDICATORS – EN 15804+A2, EF 3.1",
                "table": "CORE ENVIRONMENTAL IMPACT INDICATORS – EN 15804+A2, EF 3.1",
                "module": "B6",
                "unit_raw": "kg CO2e"
              }
            },
            "B7": {
              "value": null,
              "raw": "ND",
              "status": "not_declared",
              "provenance": {
                "page": 8,
                "section": "CORE ENVIRONMENTAL IMPACT INDICATORS – EN 15804+A2, EF 3.1",
                "table": "CORE ENVIRONMENTAL IMPACT INDICATORS – EN 15804+A2, EF 3.1",
                "module": "B7",
                "unit_raw": "kg CO2e"
              }
            },
            "C1": {
              "value": 0.000449,
              "raw": "4.49E‐04",
              "status": "declared",
              "provenance": {
                "page": 8,
                "section": "CORE ENVIRONMENTAL IMPACT INDICATORS – EN 15804+A2, EF 3.1",
                "table": "CORE ENVIRONMENTAL IMPACT INDICATORS – EN 15804+A2, EF 3.1",
                "module": "C1",
                "unit_raw": "kg CO2e"
              }
            },
            "C2": {
              "value": 0.00555,
              "raw": "5.55E‐03",
              "status": "declared",
              "provenance": {
                "page": 8,
                "section": "CORE ENVIRONMENTAL IMPACT INDICATORS – EN 15804+A2, EF 3.1",
                "table": "CORE ENVIRONMENTAL IMPACT INDICATORS – EN 15804+A2, EF 3.1",
                "module": "C2",
                "unit_raw": "kg CO2e"
              }
            },
            "C3": {
              "value": 0.000724,
              "raw": "7.24E‐04",
              "status": "declared",
              "provenance": {
                "page": 8,
                "section": "CORE ENVIRONMENTAL IMPACT INDICATORS – EN 15804+A2, EF 3.1",
                "table": "CORE ENVIRONMENTAL IMPACT INDICATORS – EN 15804+A2, EF 3.1",
                "module": "C3",
                "unit_raw": "kg CO2e"
              }
            },
            "C4": {
              "value": 0.00247,
              "raw": "2.47E‐03",
              "status": "declared",
              "provenance": {
                "page": 8,
                "section": "CORE ENVIRONMENTAL IMPACT INDICATORS – EN 15804+A2, EF 3.1",
                "table": "CORE ENVIRONMENTAL IMPACT INDICATORS – EN 15804+A2, EF 3.1",
                "module": "C4",
                "unit_raw": "kg CO2e"
              }
            },
            "D": {
              "value": -0.0164,
              "raw": "‐1.64E‐02",
              "status": "declared",
              "provenance": {
                "page": 8,
                "section": "CORE ENVIRONMENTAL IMPACT INDICATORS – EN 15804+A2, EF 3.1",
                "table": "CORE ENVIRONMENTAL IMPACT INDICATORS – EN 15804+A2, EF 3.1",
                "module": "D",
                "unit_raw": "kg CO2e"
              }
            }
          }
        },
        "GWP_total_CML": {
          "unit_raw": "kg CO2e",
          "unit_normalised": "kg CO2e",
          "header_modules": [
            "A1",
            "A2",
            "A3",
            "A1-A3",
            "A4",
            "A5",
            "B1",
            "B2",
            "B3",
            "B4",
            "B5",
            "B6",
            "B7",
            "C1",
            "C2",
            "C3",
            "C4",
            "D"
          ],
          "modules": {}
        },
        "GWP_GHG": {
          "unit_raw": "kg CO2e",
          "unit_normalised": "kg CO2e",
          "header_modules": [
            "A1",
            "A2",
            "A3",
            "A1-A3",
            "A4",
            "A5",
            "B1",
            "B2",
            "B3",
            "B4",
            "B5",
            "B6",
            "B7",
            "C1",
            "C2",
            "C3",
            "C4",
            "D"
          ],
          "modules": {
            "A1": {
              "value": 235.0,
              "raw": "2.35E+02",
              "status": "declared",
              "provenance": {
                "page": 11,
                "section": "ADDITIONAL INDICATOR – GWP-GHG",
                "table": "ADDITIONAL INDICATOR – GWP-GHG",
                "module": "A1",
                "unit_raw": "kg CO2e"
              }
            },
            "A2": {
              "value": 34.2,
              "raw": "3.42E+01",
              "status": "declared",
              "provenance": {
                "page": 11,
                "section": "ADDITIONAL INDICATOR – GWP-GHG",
                "table": "ADDITIONAL INDICATOR – GWP-GHG",
                "module": "A2",
                "unit_raw": "kg CO2e"
              }
            },
            "A3": {
              "value": 3.71,
              "raw": "3.71E+00",
              "status": "declared",
              "provenance": {
                "page": 11,
                "section": "ADDITIONAL INDICATOR – GWP-GHG",
                "table": "ADDITIONAL INDICATOR – GWP-GHG",
                "module": "A3",
                "unit_raw": "kg CO2e"
              }
            },
            "A1-A3": {
              "value": 273.0,
              "raw": "2.73E+02",
              "status": "declared",
              "provenance": {
                "page": 11,
                "section": "ADDITIONAL INDICATOR – GWP-GHG",
                "table": "ADDITIONAL INDICATOR – GWP-GHG",
                "module": "A1-A3",
                "unit_raw": "kg CO2e"
              }
            },
            "A4": {
              "value": 2.95,
              "raw": "2.95E+00",
              "status": "declared",
              "provenance": {
                "page": 11,
                "section": "ADDITIONAL INDICATOR – GWP-GHG",
                "table": "ADDITIONAL INDICATOR – GWP-GHG",
                "module": "A4",
                "unit_raw": "kg CO2e"
              }
            },
            "A5": {
              "value": 16.4,
              "raw": "1.64E+01",
              "status": "declared",
              "provenance": {
                "page": 11,
                "section": "ADDITIONAL INDICATOR – GWP-GHG",
                "table": "ADDITIONAL INDICATOR – GWP-GHG",
                "module": "A5",
                "unit_raw": "kg CO2e"
              }
            },
            "B1": {
              "value": null,
              "raw": "ND",
              "status": "not_declared",
              "provenance": {
                "page": 11,
                "section": "ADDITIONAL INDICATOR – GWP-GHG",
                "table": "ADDITIONAL INDICATOR – GWP-GHG",
                "module": "B1",
                "unit_raw": "kg CO2e"
              }
            },
            "B2": {
              "value": null,
              "raw": "ND",
              "status": "not_declared",
              "provenance": {
                "page": 11,
                "section": "ADDITIONAL INDICATOR – GWP-GHG",
                "table": "ADDITIONAL INDICATOR – GWP-GHG",
                "module": "B2",
                "unit_raw": "kg CO2e"
              }
            },
            "B3": {
              "value": null,
              "raw": "ND",
              "status": "not_declared",
              "provenance": {
                "page": 11,
                "section": "ADDITIONAL INDICATOR – GWP-GHG",
                "table": "ADDITIONAL INDICATOR – GWP-GHG",
                "module": "B3",
                "unit_raw": "kg CO2e"
              }
            },
            "B4": {
              "value": null,
              "raw": "ND",
              "status": "not_declared",
              "provenance": {
                "page": 11,
                "section": "ADDITIONAL INDICATOR – GWP-GHG",
                "table": "ADDITIONAL INDICATOR – GWP-GHG",
                "module": "B4",
                "unit_raw": "kg CO2e"
              }
            },
            "B5": {
              "value": null,
              "raw": "ND",
              "status": "not_declared",
              "provenance": {
                "page": 11,
                "section": "ADDITIONAL INDICATOR – GWP-GHG",
                "table": "ADDITIONAL INDICATOR – GWP-GHG",
                "module": "B5",
                "unit_raw": "kg CO2e"
              }
            },
            "B6": {
              "value": null,
              "raw": "ND",
              "status": "not_declared",
              "provenance": {
                "page": 11,
                "section": "ADDITIONAL INDICATOR – GWP-GHG",
                "table": "ADDITIONAL INDICATOR – GWP-GHG",
                "module": "B6",
                "unit_raw": "kg CO2e"
              }
            },
            "B7": {
              "value": null,
              "raw": "ND",
              "status": "not_declared",
              "provenance": {
                "page": 11,
                "section": "ADDITIONAL INDICATOR – GWP-GHG",
                "table": "ADDITIONAL INDICATOR – GWP-GHG",
                "module": "B7",
                "unit_raw": "kg CO2e"
              }
            },
            "C1": {
              "value": 4.39,
              "raw": "4.39E+00",
              "status": "declared",
              "provenance": {
                "page": 11,
                "section": "ADDITIONAL INDICATOR – GWP-GHG",
                "table": "ADDITIONAL INDICATOR – GWP-GHG",
                "module": "C1",
                "unit_raw": "kg CO2e"
              }
            },
            "C2": {
              "value": 12.4,
              "raw": "1.24E+01",
              "status": "declared",
              "provenance": {
                "page": 11,
                "section": "ADDITIONAL INDICATOR – GWP-GHG",
                "table": "ADDITIONAL INDICATOR – GWP-GHG",
                "module": "C2",
                "unit_raw": "kg CO2e"
              }
            },
            "C3": {
              "value": 7.06,
              "raw": "7.06E+00",
              "status": "declared",
              "provenance": {
                "page": 11,
                "section": "ADDITIONAL INDICATOR – GWP-GHG",
                "table": "ADDITIONAL INDICATOR – GWP-GHG",
                "module": "C3",
                "unit_raw": "kg CO2e"
              }
            },
            "C4": {
              "value": 4.32,
              "raw": "4.32E+00",
              "status": "declared",
              "provenance": {
                "page": 11,
                "section": "ADDITIONAL INDICATOR – GWP-GHG",
                "table": "ADDITIONAL INDICATOR – GWP-GHG",
                "module": "C4",
                "unit_raw": "kg CO2e"
              }
            },
            "D": {
              "value": -11.8,
              "raw": "‐1.18E+01",
              "status": "declared",
              "provenance": {
                "page": 11,
                "section": "ADDITIONAL INDICATOR – GWP-GHG",
                "table": "ADDITIONAL INDICATOR – GWP-GHG",
                "module": "D",
                "unit_raw": "kg CO2e"
              }
            }
          }
        }
      }
    }
  ],
  "system_boundary": {
    "A1": "declared",
    "A2": "declared",
    "A3": "declared",
    "A1-A3": "declared",
    "A4": "declared",
    "A5": "declared",
    "B1": "not_declared",
    "B2": "not_declared",
    "B3": "not_declared",
    "B4": "not_declared",
    "B5": "not_declared",
    "B6": "not_declared",
    "B7": "not_declared",
    "C1": "declared",
    "C2": "declared",
    "C3": "declared",
    "C4": "declared",
    "D": "declared"
  },
  "comparability_notes": [],
  "extraction_meta": {
    "method": "deterministic coordinate/order-bound table parse; contextual fields agent-verified",
    "numbers_validated": "cross_validate.py (raw string present on cited page)",
    "verified_by": "main-agent source-read fix",
    "checked_by": null,
    "confidence": "high",
    "warnings": [],
    "needs_review": []
  }
}