{
  "schema_version": "1.0",
  "epd": {
    "id": "EPD_HUB-5882",
    "source_pdf": "EPD_HUB-5882_2026-06-27_en.pdf",
    "pages": 20,
    "program_operator": "EPD Hub, hub@epdhub.com",
    "pcr": "EPD Hub Core PCR version 1.2, 24 Mar 2025",
    "reference_standard": "EN 15804:2012+A2:2019/AC:2021 and ISO 14025",
    "en15804_version": "A2",
    "characterisation": "EF 3.1",
    "published": "27.03.2026",
    "valid_until": "26.03.2031",
    "provenance": {
      "program_operator": {
        "page": 3,
        "snippet": "Program operator | EPD Hub, hub@epdhub.com"
      },
      "pcr": {
        "page": 3,
        "snippet": "PCR | EPD Hub Core PCR version 1.2, 24 Mar 2025"
      },
      "published": {
        "page": 1,
        "snippet": "Published on 27.03.2026"
      },
      "valid_until": {
        "page": 1,
        "snippet": "valid until 26.03.2031"
      }
    }
  },
  "products": [
    {
      "name": "40 MPa High Performance Concrete",
      "manufacturer": "Boral Limited",
      "concrete_type": "Ready-mix concrete",
      "compressive_strength": {
        "value_mpa": 40,
        "class": "S40",
        "at_days": null,
        "raw": null,
        "status": "found",
        "provenance": {
          "page": 4,
          "snippet": "Compressive strength class: | S40"
        }
      },
      "manufacturing_location": {
        "site": "Melbourne",
        "city": "Melbourne",
        "region": "Victoria",
        "country": "AU",
        "raw": "Melbourne",
        "provenance": {
          "page": 3,
          "snippet": "Manufacturer Boral Limited; Place of production Melbourne"
        }
      },
      "declared_unit": {
        "amount": 1,
        "unit": "m3",
        "description": "1 cubic metre",
        "mass_kg": 2338.0,
        "provenance": {
          "page": 4,
          "snippet": "Declared unit | 1 cubic metre"
        }
      },
      "indicators": {
        "GWP_total": {
          "unit_raw": "kg CO2e",
          "unit_normalised": "kg CO2e",
          "header_modules": [
            "A1",
            "A2",
            "A3",
            "A1-A3",
            "C1",
            "C2",
            "C3",
            "C4",
            "D"
          ],
          "modules": {
            "A1": {
              "value": 276.0,
              "raw": "2.76E+02",
              "status": "declared",
              "provenance": {
                "page": 13,
                "section": "IN ACCORDANCE WITH EN 15804+A2 & ISO 14025",
                "table": "IN ACCORDANCE WITH EN 15804+A2 & ISO 14025",
                "module": "A1",
                "unit_raw": "kg CO2e"
              }
            },
            "A2": {
              "value": 15.0,
              "raw": "1.50E+01",
              "status": "declared",
              "provenance": {
                "page": 13,
                "section": "IN ACCORDANCE WITH EN 15804+A2 & ISO 14025",
                "table": "IN ACCORDANCE WITH EN 15804+A2 & ISO 14025",
                "module": "A2",
                "unit_raw": "kg CO2e"
              }
            },
            "A3": {
              "value": 5.6,
              "raw": "5.60E+00",
              "status": "declared",
              "provenance": {
                "page": 13,
                "section": "IN ACCORDANCE WITH EN 15804+A2 & ISO 14025",
                "table": "IN ACCORDANCE WITH EN 15804+A2 & ISO 14025",
                "module": "A3",
                "unit_raw": "kg CO2e"
              }
            },
            "A1-A3": {
              "value": 297.0,
              "raw": "2.97E+02",
              "status": "declared",
              "provenance": {
                "page": 13,
                "section": "IN ACCORDANCE WITH EN 15804+A2 & ISO 14025",
                "table": "IN ACCORDANCE WITH EN 15804+A2 & ISO 14025",
                "module": "A1-A3",
                "unit_raw": "kg CO2e"
              }
            },
            "C1": {
              "value": 4.45,
              "raw": "4.45E+00",
              "status": "declared",
              "provenance": {
                "page": 14,
                "section": "IN ACCORDANCE WITH EN 15804+A2 & ISO 14025",
                "table": "IN ACCORDANCE WITH EN 15804+A2 & ISO 14025",
                "module": "C1",
                "unit_raw": "kg CO2e"
              }
            },
            "C2": {
              "value": 12.6,
              "raw": "1.26E+01",
              "status": "declared",
              "provenance": {
                "page": 14,
                "section": "IN ACCORDANCE WITH EN 15804+A2 & ISO 14025",
                "table": "IN ACCORDANCE WITH EN 15804+A2 & ISO 14025",
                "module": "C2",
                "unit_raw": "kg CO2e"
              }
            },
            "C3": {
              "value": 7.16,
              "raw": "7.16E+00",
              "status": "declared",
              "provenance": {
                "page": 14,
                "section": "IN ACCORDANCE WITH EN 15804+A2 & ISO 14025",
                "table": "IN ACCORDANCE WITH EN 15804+A2 & ISO 14025",
                "module": "C3",
                "unit_raw": "kg CO2e"
              }
            },
            "C4": {
              "value": 4.38,
              "raw": "4.38E+00",
              "status": "declared",
              "provenance": {
                "page": 14,
                "section": "IN ACCORDANCE WITH EN 15804+A2 & ISO 14025",
                "table": "IN ACCORDANCE WITH EN 15804+A2 & ISO 14025",
                "module": "C4",
                "unit_raw": "kg CO2e"
              }
            },
            "D": {
              "value": -12.8,
              "raw": "-1.28E+01",
              "status": "declared",
              "provenance": {
                "page": 14,
                "section": "IN ACCORDANCE WITH EN 15804+A2 & ISO 14025",
                "table": "IN ACCORDANCE WITH EN 15804+A2 & ISO 14025",
                "module": "D",
                "unit_raw": "kg CO2e"
              }
            }
          }
        },
        "GWP_fossil": {
          "unit_raw": "kg CO2e",
          "unit_normalised": "kg CO2e",
          "header_modules": [
            "A1",
            "A2",
            "A3",
            "A1-A3",
            "C1",
            "C2",
            "C3",
            "C4",
            "D"
          ],
          "modules": {
            "A1": {
              "value": 276.0,
              "raw": "2.76E+02",
              "status": "declared",
              "provenance": {
                "page": 13,
                "section": "IN ACCORDANCE WITH EN 15804+A2 & ISO 14025",
                "table": "IN ACCORDANCE WITH EN 15804+A2 & ISO 14025",
                "module": "A1",
                "unit_raw": "kg CO2e"
              }
            },
            "A2": {
              "value": 15.0,
              "raw": "1.50E+01",
              "status": "declared",
              "provenance": {
                "page": 13,
                "section": "IN ACCORDANCE WITH EN 15804+A2 & ISO 14025",
                "table": "IN ACCORDANCE WITH EN 15804+A2 & ISO 14025",
                "module": "A2",
                "unit_raw": "kg CO2e"
              }
            },
            "A3": {
              "value": 5.6,
              "raw": "5.60E+00",
              "status": "declared",
              "provenance": {
                "page": 13,
                "section": "IN ACCORDANCE WITH EN 15804+A2 & ISO 14025",
                "table": "IN ACCORDANCE WITH EN 15804+A2 & ISO 14025",
                "module": "A3",
                "unit_raw": "kg CO2e"
              }
            },
            "A1-A3": {
              "value": 297.0,
              "raw": "2.97E+02",
              "status": "declared",
              "provenance": {
                "page": 13,
                "section": "IN ACCORDANCE WITH EN 15804+A2 & ISO 14025",
                "table": "IN ACCORDANCE WITH EN 15804+A2 & ISO 14025",
                "module": "A1-A3",
                "unit_raw": "kg CO2e"
              }
            },
            "C1": {
              "value": 4.45,
              "raw": "4.45E+00",
              "status": "declared",
              "provenance": {
                "page": 14,
                "section": "IN ACCORDANCE WITH EN 15804+A2 & ISO 14025",
                "table": "IN ACCORDANCE WITH EN 15804+A2 & ISO 14025",
                "module": "C1",
                "unit_raw": "kg CO2e"
              }
            },
            "C2": {
              "value": 12.6,
              "raw": "1.26E+01",
              "status": "declared",
              "provenance": {
                "page": 14,
                "section": "IN ACCORDANCE WITH EN 15804+A2 & ISO 14025",
                "table": "IN ACCORDANCE WITH EN 15804+A2 & ISO 14025",
                "module": "C2",
                "unit_raw": "kg CO2e"
              }
            },
            "C3": {
              "value": 7.16,
              "raw": "7.16E+00",
              "status": "declared",
              "provenance": {
                "page": 14,
                "section": "IN ACCORDANCE WITH EN 15804+A2 & ISO 14025",
                "table": "IN ACCORDANCE WITH EN 15804+A2 & ISO 14025",
                "module": "C3",
                "unit_raw": "kg CO2e"
              }
            },
            "C4": {
              "value": 4.38,
              "raw": "4.38E+00",
              "status": "declared",
              "provenance": {
                "page": 14,
                "section": "IN ACCORDANCE WITH EN 15804+A2 & ISO 14025",
                "table": "IN ACCORDANCE WITH EN 15804+A2 & ISO 14025",
                "module": "C4",
                "unit_raw": "kg CO2e"
              }
            },
            "D": {
              "value": -12.7,
              "raw": "-1.27E+01",
              "status": "declared",
              "provenance": {
                "page": 14,
                "section": "IN ACCORDANCE WITH EN 15804+A2 & ISO 14025",
                "table": "IN ACCORDANCE WITH EN 15804+A2 & ISO 14025",
                "module": "D",
                "unit_raw": "kg CO2e"
              }
            }
          }
        },
        "GWP_biogenic": {
          "unit_raw": "kg CO2e",
          "unit_normalised": "kg CO2e",
          "header_modules": [
            "A1",
            "A2",
            "A3",
            "A1-A3",
            "C1",
            "C2",
            "C3",
            "C4",
            "D"
          ],
          "modules": {
            "A1": {
              "value": -0.00397,
              "raw": "-3.97E-03",
              "status": "declared",
              "provenance": {
                "page": 13,
                "section": "IN ACCORDANCE WITH EN 15804+A2 & ISO 14025",
                "table": "IN ACCORDANCE WITH EN 15804+A2 & ISO 14025",
                "module": "A1",
                "unit_raw": "kg CO2e"
              }
            },
            "A2": {
              "value": 0.0279,
              "raw": "2.79E-02",
              "status": "declared",
              "provenance": {
                "page": 13,
                "section": "IN ACCORDANCE WITH EN 15804+A2 & ISO 14025",
                "table": "IN ACCORDANCE WITH EN 15804+A2 & ISO 14025",
                "module": "A2",
                "unit_raw": "kg CO2e"
              }
            },
            "A3": {
              "value": 0.00076,
              "raw": "7.60E-04",
              "status": "declared",
              "provenance": {
                "page": 13,
                "section": "IN ACCORDANCE WITH EN 15804+A2 & ISO 14025",
                "table": "IN ACCORDANCE WITH EN 15804+A2 & ISO 14025",
                "module": "A3",
                "unit_raw": "kg CO2e"
              }
            },
            "A1-A3": {
              "value": 0.0247,
              "raw": "2.47E-02",
              "status": "declared",
              "provenance": {
                "page": 13,
                "section": "IN ACCORDANCE WITH EN 15804+A2 & ISO 14025",
                "table": "IN ACCORDANCE WITH EN 15804+A2 & ISO 14025",
                "module": "A1-A3",
                "unit_raw": "kg CO2e"
              }
            },
            "C1": {
              "value": 0.000454,
              "raw": "4.54E-04",
              "status": "declared",
              "provenance": {
                "page": 14,
                "section": "IN ACCORDANCE WITH EN 15804+A2 & ISO 14025",
                "table": "IN ACCORDANCE WITH EN 15804+A2 & ISO 14025",
                "module": "C1",
                "unit_raw": "kg CO2e"
              }
            },
            "C2": {
              "value": 0.00285,
              "raw": "2.85E-03",
              "status": "declared",
              "provenance": {
                "page": 14,
                "section": "IN ACCORDANCE WITH EN 15804+A2 & ISO 14025",
                "table": "IN ACCORDANCE WITH EN 15804+A2 & ISO 14025",
                "module": "C2",
                "unit_raw": "kg CO2e"
              }
            },
            "C3": {
              "value": -0.000731,
              "raw": "-7.31E-04",
              "status": "declared",
              "provenance": {
                "page": 14,
                "section": "IN ACCORDANCE WITH EN 15804+A2 & ISO 14025",
                "table": "IN ACCORDANCE WITH EN 15804+A2 & ISO 14025",
                "module": "C3",
                "unit_raw": "kg CO2e"
              }
            },
            "C4": {
              "value": -0.00139,
              "raw": "-1.39E-03",
              "status": "declared",
              "provenance": {
                "page": 14,
                "section": "IN ACCORDANCE WITH EN 15804+A2 & ISO 14025",
                "table": "IN ACCORDANCE WITH EN 15804+A2 & ISO 14025",
                "module": "C4",
                "unit_raw": "kg CO2e"
              }
            },
            "D": {
              "value": -0.04,
              "raw": "-4.00E-02",
              "status": "declared",
              "provenance": {
                "page": 14,
                "section": "IN ACCORDANCE WITH EN 15804+A2 & ISO 14025",
                "table": "IN ACCORDANCE WITH EN 15804+A2 & ISO 14025",
                "module": "D",
                "unit_raw": "kg CO2e"
              }
            }
          }
        },
        "GWP_luluc": {
          "unit_raw": "kg CO2e",
          "unit_normalised": "kg CO2e",
          "header_modules": [
            "A1",
            "A2",
            "A3",
            "A1-A3",
            "C1",
            "C2",
            "C3",
            "C4",
            "D"
          ],
          "modules": {
            "A1": {
              "value": 0.0474,
              "raw": "4.74E-02",
              "status": "declared",
              "provenance": {
                "page": 13,
                "section": "IN ACCORDANCE WITH EN 15804+A2 & ISO 14025",
                "table": "IN ACCORDANCE WITH EN 15804+A2 & ISO 14025",
                "module": "A1",
                "unit_raw": "kg CO2e"
              }
            },
            "A2": {
              "value": 0.000115,
              "raw": "1.15E-04",
              "status": "declared",
              "provenance": {
                "page": 13,
                "section": "IN ACCORDANCE WITH EN 15804+A2 & ISO 14025",
                "table": "IN ACCORDANCE WITH EN 15804+A2 & ISO 14025",
                "module": "A2",
                "unit_raw": "kg CO2e"
              }
            },
            "A3": {
              "value": 0.00046,
              "raw": "4.60E-04",
              "status": "declared",
              "provenance": {
                "page": 13,
                "section": "IN ACCORDANCE WITH EN 15804+A2 & ISO 14025",
                "table": "IN ACCORDANCE WITH EN 15804+A2 & ISO 14025",
                "module": "A3",
                "unit_raw": "kg CO2e"
              }
            },
            "A1-A3": {
              "value": 0.048,
              "raw": "4.80E-02",
              "status": "declared",
              "provenance": {
                "page": 13,
                "section": "IN ACCORDANCE WITH EN 15804+A2 & ISO 14025",
                "table": "IN ACCORDANCE WITH EN 15804+A2 & ISO 14025",
                "module": "A1-A3",
                "unit_raw": "kg CO2e"
              }
            },
            "C1": {
              "value": 0.000456,
              "raw": "4.56E-04",
              "status": "declared",
              "provenance": {
                "page": 14,
                "section": "IN ACCORDANCE WITH EN 15804+A2 & ISO 14025",
                "table": "IN ACCORDANCE WITH EN 15804+A2 & ISO 14025",
                "module": "C1",
                "unit_raw": "kg CO2e"
              }
            },
            "C2": {
              "value": 0.00563,
              "raw": "5.63E-03",
              "status": "declared",
              "provenance": {
                "page": 14,
                "section": "IN ACCORDANCE WITH EN 15804+A2 & ISO 14025",
                "table": "IN ACCORDANCE WITH EN 15804+A2 & ISO 14025",
                "module": "C2",
                "unit_raw": "kg CO2e"
              }
            },
            "C3": {
              "value": 0.000734,
              "raw": "7.34E-04",
              "status": "declared",
              "provenance": {
                "page": 14,
                "section": "IN ACCORDANCE WITH EN 15804+A2 & ISO 14025",
                "table": "IN ACCORDANCE WITH EN 15804+A2 & ISO 14025",
                "module": "C3",
                "unit_raw": "kg CO2e"
              }
            },
            "C4": {
              "value": 0.0025,
              "raw": "2.50E-03",
              "status": "declared",
              "provenance": {
                "page": 14,
                "section": "IN ACCORDANCE WITH EN 15804+A2 & ISO 14025",
                "table": "IN ACCORDANCE WITH EN 15804+A2 & ISO 14025",
                "module": "C4",
                "unit_raw": "kg CO2e"
              }
            },
            "D": {
              "value": -0.0176,
              "raw": "-1.76E-02",
              "status": "declared",
              "provenance": {
                "page": 14,
                "section": "IN ACCORDANCE WITH EN 15804+A2 & ISO 14025",
                "table": "IN ACCORDANCE WITH EN 15804+A2 & ISO 14025",
                "module": "D",
                "unit_raw": "kg CO2e"
              }
            }
          }
        },
        "GWP_GHG": {
          "unit_raw": "",
          "unit_normalised": "kg CO2e",
          "header_modules": [
            "C1",
            "C2",
            "C3",
            "C4",
            "D"
          ],
          "modules": {
            "C1": {
              "value": 276.0,
              "raw": "2.76E+02",
              "status": "declared",
              "provenance": {
                "page": 18,
                "section": "IN ACCORDANCE WITH EN 15804+A2 & ISO 14025",
                "table": "IN ACCORDANCE WITH EN 15804+A2 & ISO 14025",
                "module": "C1",
                "unit_raw": ""
              }
            },
            "C2": {
              "value": 15.0,
              "raw": "1.50E+01",
              "status": "declared",
              "provenance": {
                "page": 18,
                "section": "IN ACCORDANCE WITH EN 15804+A2 & ISO 14025",
                "table": "IN ACCORDANCE WITH EN 15804+A2 & ISO 14025",
                "module": "C2",
                "unit_raw": ""
              }
            },
            "C4": {
              "value": 5.6,
              "raw": "5.60E+00",
              "status": "declared",
              "provenance": {
                "page": 18,
                "section": "IN ACCORDANCE WITH EN 15804+A2 & ISO 14025",
                "table": "IN ACCORDANCE WITH EN 15804+A2 & ISO 14025",
                "module": "C4",
                "unit_raw": ""
              }
            },
            "D": {
              "value": 297.0,
              "raw": "2.97E+02",
              "status": "declared",
              "provenance": {
                "page": 18,
                "section": "IN ACCORDANCE WITH EN 15804+A2 & ISO 14025",
                "table": "IN ACCORDANCE WITH EN 15804+A2 & ISO 14025",
                "module": "D",
                "unit_raw": ""
              }
            },
            "C3": {
              "value": 7.16,
              "raw": "7.16E+00",
              "status": "declared",
              "provenance": {
                "page": 18,
                "section": "IN ACCORDANCE WITH EN 15804+A2 & ISO 14025",
                "table": "IN ACCORDANCE WITH EN 15804+A2 & ISO 14025",
                "module": "C3",
                "unit_raw": ""
              }
            }
          }
        }
      }
    }
  ],
  "system_boundary": {
    "A1": "declared",
    "A2": "declared",
    "A3": "declared",
    "A1-A3": "declared",
    "A4": "not_declared",
    "A5": "not_declared",
    "B1": "not_declared",
    "B2": "not_declared",
    "B3": "not_declared",
    "B4": "not_declared",
    "B5": "not_declared",
    "B6": "not_declared",
    "B7": "not_declared",
    "C1": "declared",
    "C2": "declared",
    "C3": "declared",
    "C4": "declared",
    "D": "declared"
  },
  "comparability_notes": [],
  "extraction_meta": {
    "method": "deterministic coordinate/order-bound table parse; contextual fields agent-verified",
    "numbers_validated": "cross_validate.py (raw string present on cited page)",
    "verified_by": "main-agent source-read fix",
    "checked_by": null,
    "confidence": "high",
    "warnings": [
      "Cell conflict across pages: GWP_GHG.C1: '2.76E+02' vs '4.45E+00'",
      "Cell conflict across pages: GWP_GHG.C2: '1.50E+01' vs '1.26E+01'",
      "Cell conflict across pages: GWP_GHG.C4: '5.60E+00' vs '4.38E+00'",
      "Cell conflict across pages: GWP_GHG.D: '2.97E+02' vs '-1.27E+01'"
    ],
    "needs_review": []
  }
}